Started adding namespaces.  It makes the declarations of a few functions ugly.  I'll see if I can go clean those up later.

SoftwareFoundations/LogicalFoundations/Imp.lean
@@ -6,56 +6,607 @@ import Mathlib.tactic.linarith
 
 import «SoftwareFoundations».«LogicalFoundations».«Maps»
 
-/-
-## Arithmetic and Boolean Expressions
--/
+namespace SoftwareFoundations.LogicalFoundations.Imp
+  /-
+  ## Arithmetic and Boolean Expressions
+  -/
 
-/-
-### Syntax
--/
+  /-
+  ### Syntax
+  -/
 
-namespace AExp
+  namespace AExp
+    inductive Arith: Type where
+      | num (n: Nat): Arith
+      | plus (e₁ e₂: Arith): Arith
+      | minus (e₁ e₂: Arith): Arith
+      | mult (e₁ e₂: Arith): Arith
+
+    @[reducible]
+    def Arith.eval: Arith → Nat
+      | .num n => n
+      | .plus e₁ e₂ => e₁.eval + e₂.eval
+      | .minus e₁ e₂ => e₁.eval - e₂.eval
+      | .mult e₁ e₂ => e₁.eval * e₂.eval
+
+    @[reducible]
+    def Arith.optZeroPlus: Arith → Arith
+      | .num n => .num n
+      | .plus (.num 0) e₂ => e₂.optZeroPlus
+      | .plus e₁ e₂ => .plus e₁.optZeroPlus e₂.optZeroPlus
+      | .minus e₁ e₂ => .minus e₁.optZeroPlus e₂.optZeroPlus
+      | .mult e₁ e₂ => .mult e₁.optZeroPlus e₂.optZeroPlus
+
+    example: (Arith.plus (.num 2) (.num 2)).eval = 4 := rfl
+    example: (Arith.plus (.num 2) (.plus (.num 0) (.plus (.num 0) (.num 1)))).optZeroPlus = .plus (.num 2) (.num 1) := rfl
+
+    example: (a: Arith) → a.optZeroPlus.eval = a.eval
+      | .num _ => rfl
+      | .plus e₁ e₂ =>
+        have ih₁: e₁.optZeroPlus.eval = e₁.eval := _example e₁
+        have ih₂: e₂.optZeroPlus.eval = e₂.eval := _example e₂
+        match e₁ with
+          | .num n =>
+            match n with
+              | .zero =>
+                calc (Arith.plus (.num 0) e₂).optZeroPlus.eval
+                  _ = e₂.optZeroPlus.eval                := rfl
+                  _ = e₂.eval                            := ih₂
+                  _ = 0 + e₂.eval                        := Eq.symm (Nat.zero_add e₂.eval)
+              | .succ n =>
+                calc (Arith.plus (.num n.succ) e₂).optZeroPlus.eval
+                  _ = (Arith.num n.succ).optZeroPlus.eval + e₂.optZeroPlus.eval := rfl
+                  _ = (Arith.num n.succ).eval + e₂.eval                         := congr (congrArg Nat.add ih₁) ih₂
+          | .plus _ _ =>
+            calc (Arith.plus (Arith.plus _ _) e₂).optZeroPlus.eval
+              _ = (Arith.plus _ _).optZeroPlus.eval + e₂.optZeroPlus.eval := rfl
+              _ = (Arith.plus _ _).eval + e₂.eval                         := congr (congrArg Nat.add ih₁) ih₂
+          | .minus _ _ =>
+            calc (Arith.plus (Arith.minus _ _) e₂).optZeroPlus.eval
+              _ = (Arith.minus _ _).optZeroPlus.eval + e₂.optZeroPlus.eval := rfl
+              _ = (Arith.minus _ _).eval + e₂.eval                         := congr (congrArg Nat.add ih₁) ih₂
+          | .mult _ _ =>
+            calc (Arith.plus (Arith.mult _ _) e₂).optZeroPlus.eval
+              _ = (Arith.mult _ _).optZeroPlus.eval + e₂.optZeroPlus.eval := rfl
+              _ = (Arith.mult _ _).eval + e₂.eval                         := congr (congrArg Nat.add ih₁) ih₂
+      | .minus e₁ e₂ =>
+        have ih₁: e₁.optZeroPlus.eval = e₁.eval := _example e₁
+        have ih₂: e₂.optZeroPlus.eval = e₂.eval := _example e₂
+        calc (Arith.minus e₁ e₂).optZeroPlus.eval
+          _ = e₁.optZeroPlus.eval - e₂.optZeroPlus.eval := rfl
+          _ = e₁.eval - e₂.eval                         := congr (congrArg Nat.sub ih₁) ih₂
+      | .mult e₁ e₂ =>
+        have ih₁: e₁.optZeroPlus.eval = e₁.eval := _example e₁
+        have ih₂: e₂.optZeroPlus.eval = e₂.eval := _example e₂
+        calc (Arith.mult e₁ e₂).optZeroPlus.eval
+          _ = e₁.optZeroPlus.eval * e₂.optZeroPlus.eval := rfl
+          _ = e₁.eval * e₂.eval                         := congr (congrArg Nat.mul ih₁) ih₂
+          _ = (Arith.mult e₁ e₂).eval                   := rfl
+
+    theorem Arith.optZeroPlus.sound (a: Arith): a.optZeroPlus.eval = a.eval := by
+      induction a with
+        | num n => rfl
+        | plus e₁ e₂ ih₁ ih₂ =>
+          cases e₁ with
+            | num n =>
+              cases n with
+                | zero => simp_all
+                | succ n =>
+                  unfold optZeroPlus eval
+                  simp_all
+            | plus | minus | mult =>
+              unfold optZeroPlus eval
+              simp_all
+        | minus _ _ ih₁ ih₂ | mult _ _ ih₁ ih₂ =>
+          unfold optZeroPlus eval
+          simp_all
+
+    example: (a: Arith) → a.optZeroPlus.eval = a.eval
+      | .num _ => by rfl
+      | .plus e₁ e₂ =>
+        have ih₁: e₁.optZeroPlus.eval = e₁.eval := _example e₁
+        have ih₂: e₂.optZeroPlus.eval = e₂.eval := _example e₂
+        match e₁ with
+          | .num n =>
+            match n with
+              | .zero =>
+                calc (Arith.plus (.num 0) e₂).optZeroPlus.eval
+                  _ = e₂.optZeroPlus.eval                := by rfl
+                  _ = e₂.eval                            := by rw [ih₂]
+                  _ = 0 + e₂.eval                        := by rw [Nat.zero_add]
+              | .succ n =>
+                calc (Arith.plus (.num n.succ) e₂).optZeroPlus.eval
+                  _ = (Arith.num n.succ).optZeroPlus.eval + e₂.optZeroPlus.eval := by rfl
+                  _ = (Arith.num n.succ).eval + e₂.eval                         := by rw [ih₁, ih₂]
+          | .plus _ _ | .minus _ _ | .mult _ _ => by
+            unfold Arith.eval
+            rw [ih₁, ih₂]
+      | .minus e₁ e₂ | .mult e₁ e₂ => by
+        have ih₁: e₁.optZeroPlus.eval = e₁.eval := _example e₁
+        have ih₂: e₂.optZeroPlus.eval = e₂.eval := _example e₂
+        unfold Arith.eval
+        rw [ih₁, ih₂]
+
+    inductive Logic: Type where
+      | true: Logic
+      | false: Logic
+      | eq (e₁ e₂: Arith): Logic
+      | neq (e₁ e₂: Arith): Logic
+      | le (e₁ e₂: Arith): Logic
+      | gt (e₁ e₂: Arith): Logic
+      | not (e: Logic): Logic
+      | and (e₁ e₂: Logic): Logic
+
+    @[reducible]
+    def Logic.eval: Logic → Bool
+      | .true => Bool.true
+      | .false => Bool.false
+      | .eq e₁ e₂ => e₁.eval == e₂.eval
+      | .neq e₁ e₂ => e₁.eval != e₂.eval
+      | .le e₁ e₂ => e₁.eval ≤ e₂.eval
+      | .gt e₁ e₂ => e₁.eval > e₂.eval
+      | .not e => !e.eval
+      | .and e₁ e₂ => e₁.eval && e₂.eval
+
+    @[reducible]
+    def Logic.optZeroPlus: Logic → Logic
+      | .true => .true
+      | .false => .false
+      | .eq e₁ e₂ => .eq e₁.optZeroPlus e₂.optZeroPlus
+      | .neq e₁ e₂ => .neq e₁.optZeroPlus e₂.optZeroPlus
+      | .le e₁ e₂ => .le e₁.optZeroPlus e₂.optZeroPlus
+      | .gt e₁ e₂ => .gt e₁.optZeroPlus e₂.optZeroPlus
+      | .not e => .not e.optZeroPlus
+      | .and e₁ e₂ => .and e₁.optZeroPlus e₂.optZeroPlus
+
+    /-
+    ## Lean (Coq) Automation
+    -/
+
+    /-
+    ### The `try` Tactical
+    -/
+
+    example (P: Prop) (h: P): P := by
+      try rfl
+      apply h
+
+    example (a: Arith): a.eval = a.eval := by
+      try rfl
+
+    /-
+    ### The `<;>` Tactical (Simple Form)
+    -/
+
+    example (n: Nat): 0 ≤ n := by
+      cases n with
+        | zero => simp
+        | succ n => simp
+
+    example (n: Nat): 0 ≤ n := by
+      cases n <;> simp
+
+    /-
+    ### The `<;>` Tactical (General Form)
+    -/
+
+    example (a: Arith): a.optZeroPlus.eval = a.eval := by
+      induction a <;>
+      try (first | rfl
+                 | unfold Arith.optZeroPlus Arith.eval
+                   simp_all)
+      case plus e₁ _ ih₁ ih₂ =>
+        cases e₁ <;>
+        try (unfold Arith.optZeroPlus Arith.eval
+             rw [ih₁, ih₂])
+        case num n =>
+          cases n with
+            | zero => simp_all
+            | succ n =>
+              unfold Arith.optZeroPlus Arith.eval
+              simp_all
+
+    /-
+    ### The `repeat` Tactical
+    -/
+
+    def In (x: α) (l: List α): Prop :=
+      match l with
+        | [] => False
+        | b :: m => b = x ∨ In x m
+
+    example: In 10 [1, 2, 3, 4, 5, 6, 7, 8, 9, 10] := by
+      repeat (try (first | apply Or.inl; rfl | apply Or.inr))
+
+    example: (b: Logic) → b.optZeroPlus.eval = b.eval
+      | .true | .false => rfl
+      | .eq e₁ e₂ =>
+        have h₁ := Arith.optZeroPlus.sound e₁
+        have h₂ := Arith.optZeroPlus.sound e₂
+        calc (Logic.eq e₁ e₂).optZeroPlus.eval
+          _ = BEq.beq e₁.optZeroPlus.eval e₂.optZeroPlus.eval := rfl
+          _ = BEq.beq e₁.eval e₂.eval                         := congr (congrArg BEq.beq h₁) h₂
+      | .neq e₁ e₂ =>
+        have h₁ := Arith.optZeroPlus.sound e₁
+        have h₂ := Arith.optZeroPlus.sound e₂
+        calc (Logic.neq e₁ e₂).optZeroPlus.eval
+          _ = not (BEq.beq e₁.optZeroPlus.eval e₂.optZeroPlus.eval) := rfl
+          _ = not (BEq.beq e₁.eval e₂.eval)                         := congrArg not (congr (congrArg BEq.beq h₁) h₂)
+      | .le e₁ e₂ =>
+        have h₁ := Arith.optZeroPlus.sound e₁
+        have h₂ := Arith.optZeroPlus.sound e₂
+        calc (Logic.le e₁ e₂).optZeroPlus.eval
+          _ = (LE.le e₁.optZeroPlus.eval e₂.optZeroPlus.eval: Bool) := rfl
+          _ = (LE.le e₁.eval e₂.eval: Bool)                         := sorry -- congr (congrArg LE.le h₁) h₂
+      | .gt e₁ e₂ =>
+        have h₁ := Arith.optZeroPlus.sound e₁
+        have h₂ := Arith.optZeroPlus.sound e₂
+        calc (Logic.gt e₁ e₂).optZeroPlus.eval
+          _ = (GT.gt e₁.optZeroPlus.eval e₂.optZeroPlus.eval: Bool) := rfl
+          _ = (GT.gt e₁.eval e₂.eval: Bool)                         := sorry -- congr (congrArg LE.le h₁) h₂
+      | .not b =>
+        have ih := _example b
+        calc (Logic.not b).optZeroPlus.eval
+          _ = not b.optZeroPlus.eval := rfl
+          _ = not b.eval             := congrArg not ih
+      | .and b₁ b₂ =>
+        have ih₁ := _example b₁
+        have ih₂ := _example b₂
+        calc (Logic.and b₁ b₂).optZeroPlus.eval
+          _ = and b₁.optZeroPlus.eval b₂.optZeroPlus.eval := rfl
+          _ = and b₁.eval b₂.eval                         := congr (congrArg and ih₁) ih₂
+
+    theorem Logic.optZeroPlus.sound (e: Logic): e.optZeroPlus.eval = e.eval := by
+      induction e <;>
+      try (first | rfl
+                 | unfold Logic.optZeroPlus Logic.eval
+                   simp [Arith.optZeroPlus.sound])
+      case not e ih =>
+        unfold Logic.optZeroPlus Logic.eval
+        rw [ih]
+      case and e₁ e₂ ih₁ ih₂ =>
+        unfold Logic.optZeroPlus Logic.eval
+        rw [ih₁, ih₂]
+
+    example: (b: Logic) → b.optZeroPlus.eval = b.eval
+      | .true | .false => by rfl
+      | .eq e₁ e₂ | .neq e₁ e₂ | .le e₁ e₂ | .gt e₁ e₂ => by
+        have h₁ := Arith.optZeroPlus.sound e₁
+        have h₂ := Arith.optZeroPlus.sound e₂
+        unfold Logic.eval
+        rw [h₁, h₂]
+      | .not b => by
+        have ih := _example b
+        unfold Logic.eval
+        rw [ih]
+      | .and b₁ b₂ => by
+        have ih₁ := _example b₁
+        have ih₂ := _example b₂
+        unfold Logic.eval
+        rw [ih₁, ih₂]
+
+    @[reducible]
+    def Arith.constFold: Arith → Arith
+      | .plus e₁ e₂ =>
+        match e₁.constFold, e₂.constFold with
+          | .num n₁, .num n₂ => .num (n₁ + n₂)
+          | e₁, e₂ => .plus e₁ e₂
+      | .minus e₁ e₂ =>
+        match e₁.constFold, e₂.constFold with
+          | .num n₁, .num n₂ => .num (n₁ - n₂)
+          | e₁, e₂ => .minus e₁ e₂
+      | .mult e₁ e₂ =>
+        match e₁.constFold, e₂.constFold with
+          | .num n₁, .num n₂ => .num (n₁ * n₂)
+          | e₁, e₂ => .mult e₁ e₂
+      | e => e
+
+    -- MOAR OPTIMIZATION: Constant Folding
+
+    -- TODO: Remove Tactic Blocks
+    example: (e: Arith) → e.constFold.eval = e.eval
+      | .num _ => rfl
+      | .plus e₁ e₂ =>
+        have ih₁ := _example e₁
+        have ih₂ := _example e₂
+        match h₁: e₁.constFold with
+          | .num n₁ =>
+            match h₂: e₂.constFold with
+              | .num n₂ =>
+                calc (Arith.plus e₁ e₂).constFold.eval
+                  _ = (Arith.plus (Arith.num n₁) (Arith.num n₂)).eval := by unfold Arith.constFold; rw [h₁, h₂]
+                  _ = (Arith.num n₁).eval + (Arith.num n₂).eval       := by rfl
+                  _ = e₁.constFold.eval + e₂.constFold.eval           := by rw [h₁, h₂]
+                  _ = e₁.eval + e₂.eval                               := by rw [ih₁, ih₂]
+              | .plus _ _ =>
+                calc (Arith.plus e₁ e₂).constFold.eval
+                  _ = (Arith.plus (Arith.num n₁) (Arith.plus _ _)).eval := by unfold Arith.constFold; rw [h₁, h₂]
+                  _ = (Arith.num n₁).eval + (Arith.plus _ _).eval       := by rfl
+                  _ = e₁.constFold.eval + e₂.constFold.eval             := by rw [h₁, h₂]
+                  _ = e₁.eval + e₂.eval                                 := by rw [ih₁, ih₂]
+              | .minus _ _ =>
+                calc (Arith.plus e₁ e₂).constFold.eval
+                  _ = (Arith.plus (Arith.num n₁) (Arith.minus _ _)).eval := by unfold Arith.constFold; rw [h₁, h₂]
+                  _ = (Arith.num n₁).eval + (Arith.minus _ _).eval       := by rfl
+                  _ = e₁.constFold.eval + e₂.constFold.eval              := by rw [h₁, h₂]
+                  _ = e₁.eval + e₂.eval                                  := by rw [ih₁, ih₂]
+              | .mult _ _ =>
+                calc (Arith.plus e₁ e₂).constFold.eval
+                  _ = (Arith.plus (Arith.num n₁) (Arith.mult _ _)).eval := by unfold Arith.constFold; rw [h₁, h₂]
+                  _ = (Arith.num n₁).eval + (Arith.mult _ _).eval       := by rfl
+                  _ = e₁.constFold.eval + e₂.constFold.eval             := by rw [h₁, h₂]
+                  _ = e₁.eval + e₂.eval                                 := by rw [ih₁, ih₂]
+          | _ => sorry
+      | _ => sorry
+
+    theorem Arith.constFold.sound (e: Arith): e.constFold.eval = e.eval := by sorry
+
+    example: (e: Arith) → e.constFold.eval = e.eval
+      | .num _ => rfl
+      | .plus e₁ e₂ =>
+        have ih₁ := _example e₁
+        have ih₂ := _example e₂
+        match h₁: e₁.constFold with
+          | .num n₁ =>
+            match h₂: e₂.constFold with
+              | .num n₂ =>
+                calc (Arith.plus e₁ e₂).constFold.eval
+                  _ = (Arith.plus (Arith.num n₁) (Arith.num n₂)).eval := by unfold Arith.constFold; rw [h₁, h₂]
+                  _ = (Arith.num n₁).eval + (Arith.num n₂).eval       := by rfl
+                  _ = e₁.constFold.eval + e₂.constFold.eval           := by rw [h₁, h₂]
+                  _ = e₁.eval + e₂.eval                               := by rw [ih₁, ih₂]
+              | .plus _ _ =>
+                calc (Arith.plus e₁ e₂).constFold.eval
+                  _ = (Arith.plus (Arith.num n₁) (Arith.plus _ _)).eval := by unfold Arith.constFold; rw [h₁, h₂]
+                  _ = (Arith.num n₁).eval + (Arith.plus _ _).eval       := by rfl
+                  _ = e₁.constFold.eval + e₂.constFold.eval             := by rw [h₁, h₂]
+                  _ = e₁.eval + e₂.eval                                 := by rw [ih₁, ih₂]
+              | .minus _ _ =>
+                calc (Arith.plus e₁ e₂).constFold.eval
+                  _ = (Arith.plus (Arith.num n₁) (Arith.minus _ _)).eval := by unfold Arith.constFold; rw [h₁, h₂]
+                  _ = (Arith.num n₁).eval + (Arith.minus _ _).eval       := by rfl
+                  _ = e₁.constFold.eval + e₂.constFold.eval              := by rw [h₁, h₂]
+                  _ = e₁.eval + e₂.eval                                  := by rw [ih₁, ih₂]
+              | .mult _ _ =>
+                calc (Arith.plus e₁ e₂).constFold.eval
+                  _ = (Arith.plus (Arith.num n₁) (Arith.mult _ _)).eval := by unfold Arith.constFold; rw [h₁, h₂]
+                  _ = (Arith.num n₁).eval + (Arith.mult _ _).eval       := by rfl
+                  _ = e₁.constFold.eval + e₂.constFold.eval             := by rw [h₁, h₂]
+                  _ = e₁.eval + e₂.eval                                 := by rw [ih₁, ih₂]
+          | _ => sorry
+      | _ => sorry
+
+
+    def Logic.constFold: Logic → Logic
+      | .eq e₁ e₂ =>
+        match e₁.constFold, e₂.constFold with
+          | .num n₁, .num n₂ => if n₁ == n₂ then .true else .false
+          | e₁, e₂ => .eq e₁ e₂
+      | .neq e₁ e₂ =>
+        match e₁.constFold, e₂.constFold with
+          | .num n₁, .num n₂ => if n₁ != n₂ then .true else .false
+          | e₁, e₂ => .neq e₁ e₂
+      | .le e₁ e₂ =>
+        match e₁.constFold, e₂.constFold with
+          | .num n₁, .num n₂ => if n₁ ≤ n₂ then .true else .false
+          | e₁, e₂ => .le e₁ e₂
+      | .gt e₁ e₂ =>
+        match e₁.constFold, e₂.constFold with
+          | .num n₁, .num n₂ => if n₁ > n₂ then .true else .false
+          | e₁, e₂ => .gt e₁ e₂
+      | .not b =>
+        match b.constFold with
+          | .true => .false
+          | .false => .true
+          | b => .not b
+      | .and b₁ b₂ =>
+        match b₁.constFold, b₂.constFold with
+          | .true, .true => .true
+          | .true, .false | .false, .true | .false, .false => .false
+          | b₁, b₂ => .and b₁ b₂
+      | b => b
+
+    example: (b: Logic) → b.constFold.eval = b.eval := sorry
+    theorem Logic.constFold.sound (b: Logic): b.constFold.eval = b.eval := by sorry
+    example: (b: Logic) → b.constFold.eval = b.eval := sorry
+
+    /-
+    ## Defining New Tactics
+    -/
+
+    -- TODO: Research defining tactics in Lean
+
+    /-
+    ## The `linearith` (`lia`) Tactic
+    -/
+
+    -- import Mathlib.tactics.linarith
+
+    example (n₁ n₂ n₃ n₄: Nat) (h: n₁ + n₂ ≤ n₂ + n₃ ∧ n₃ + 3 = n₄ + 3): n₁ ≤ n₄ := by
+      linarith
+
+    example (n₁ n₂: Nat): n₁ + n₂ = n₂ + n₁ := by
+      linarith
+
+    example (n₁ n₂ n₃: Nat): n₁ + (n₂ + n₃) = (n₁ + n₂) + n₃ := by
+      linarith
+
+    /-
+    ## A Few More Handy Tactics
+    -/
+
+    -- TODO: Research the same tactics in Lean
+
+    /-
+    ## Evaluation as a Relation
+    -/
+
+    inductive ArithEval: Arith → Nat → Prop where
+      | num (n: Nat): ArithEval (.num n) n
+      | plus (e₁ e₂: Arith) (n₁ n₂: Nat) (h₁: ArithEval e₁ n₁) (h₂: ArithEval e₂ n₂): ArithEval (.plus e₁ e₂) (n₁ + n₂)
+      | minus (e₁ e₂: Arith) (n₁ n₂: Nat) (h₁: ArithEval e₁ n₁) (h₂: ArithEval e₂ n₂): ArithEval (.minus e₁ e₂) (n₁ - n₂)
+      | mult (e₁ e₂: Arith) (n₁ n₂: Nat) (h₁: ArithEval e₁ n₁) (h₂: ArithEval e₂ n₂): ArithEval (.mult e₁ e₂) (n₁ * n₂)
+
+    /-
+    ### Inference Rule Notation
+    -/
+
+    inductive LogicEval: Logic → Bool → Prop where
+      | true: LogicEval .true true
+      | false: LogicEval .false false
+      | eq (e₁ e₂: Arith) (n₁ n₂: Nat) (h₁: ArithEval e₁ n₁) (h₂: ArithEval e₂ n₂): LogicEval (.eq e₁ e₂) (n₁ == n₂)
+      | neq (e₁ e₂: Arith) (n₁ n₂: Nat) (h₁: ArithEval e₁ n₁) (h₂: ArithEval e₂ n₂): LogicEval (.neq e₁ e₂) (n₁ != n₂)
+      | le (e₁ e₂: Arith) (n₁ n₂: Nat) (h₁: ArithEval e₁ n₁) (h₂: ArithEval e₂ n₂): LogicEval (.neq e₁ e₂) (n₁ ≤ n₂)
+      | gt (e₁ e₂: Arith) (n₁ n₂: Nat) (h₁: ArithEval e₁ n₁) (h₂: ArithEval e₂ n₂): LogicEval (.neq e₁ e₂) (n₁ > n₂)
+      | not (e: Logic) (b: Bool) (h: LogicEval e b): LogicEval (.not e) !b
+      | and (e₁ e₂: Logic) (b₁ b₂: Bool) (h₁: LogicEval e₁ b₁) (h₂: LogicEval e₂ b₂): LogicEval (.and e₁ e₂) (b₁ && b₂)
+
+    /-
+    ### Equivalence of Definitions
+    -/
+
+    example {e: Arith} {n: Nat}: ArithEval e n ↔ e.eval = n :=
+      ⟨mp, mpr⟩
+      where
+        mp {e: Arith} {n: Nat}: ArithEval e n → e.eval = n
+          | .num n => rfl
+          | .plus _ _ _ _ h₁ h₂ => mpf (mp h₁) (mp h₂) Nat.add rfl
+          | .minus _ _ _ _ h₁ h₂ => mpf (mp h₁) (mp h₂) Nat.sub rfl
+          | .mult _ _ _ _ h₁ h₂ => mpf (mp h₁) (mp h₂) Nat.mul rfl
+        mpf {e e₁ e₂: Arith} {n₁ n₂: Nat} (ih₁: e₁.eval = n₁) (ih₂: e₂.eval = n₂) (f: Nat → Nat → Nat) (h: e.eval = f e₁.eval e₂.eval) :=
+          calc e.eval
+              _ = f (Arith.eval e₁) (Arith.eval e₂) := h
+              _ = f n₁ n₂                           := congr (congrArg f ih₁) ih₂
+        mpr {e: Arith} {n: Nat} (h: e.eval = n): ArithEval e n := sorry
+          -- match e with
+          --   | Arith.num _ => sorry --ArithEval.num _
+          --   | Arith.plus e₁ e₂ =>
+          --     have ih₁: sorry := sorry --mpr _
+          --     have ih₂: sorry := sorry --mpr _
+          --     sorry
+          --   | _ => sorry
+
+    theorem arith_eval_eval (a: Arith) (n: Nat): ArithEval a n ↔ a.eval = n := by
+      apply Iff.intro
+      · intro h
+        induction h <;> first | rfl
+                              | unfold Arith.eval
+                                simp_all
+      · intro h₁
+        -- generalize n = q
+        induction a with
+          | num n =>
+            rw [← h₁]
+            apply ArithEval.num
+          | plus e₁ e₂ ih₁ ih₂ =>
+            -- unfold Arith.eval at h₁
+            sorry
+          | _ => sorry
+
+    theorem logic_eval_eval (l: Logic) (b: Bool): LogicEval l b ↔ l.eval = b := by
+      apply Iff.intro
+      · intro h
+        induction h with
+          | true => rfl
+          | false => rfl
+          | eq e₁ e₂ n₁ n₂ h₁ h₂ =>
+            unfold Logic.eval
+            rw [arith_eval_eval] at *
+            simp_all
+          | neq e₁ e₂ n₁ n₂ h₁ h₂ =>
+            unfold Logic.eval
+            rw [arith_eval_eval] at *
+            simp_all
+          | le e₁ e₂ n₁ n₂ h₁ h₂ =>
+            unfold Logic.eval
+            rw [arith_eval_eval] at *
+            simp_all
+            sorry
+          | gt e₁ e₂ n₁ n₂ h₁ h₂ =>
+            unfold Logic.eval
+            rw [arith_eval_eval] at *
+            simp_all
+            sorry
+          | not e b h ih =>
+            unfold Logic.eval
+            rw [ih]
+          | and e₁ e₂ b₁ b₂ h₁ h₂ ih₁ ih₂ =>
+            unfold Logic.eval
+            rw [ih₁, ih₂]
+      · intro h
+        induction l with
+          | true =>
+            cases b with
+              | true => exact LogicEval.true
+              | false => contradiction
+          | false =>
+            cases b with
+              | true => contradiction
+              | false => exact LogicEval.false
+          | eq e₁ e₂ =>
+            unfold Logic.eval at h
+            sorry
+          -- Other Arith cases
+          | not e ih => sorry
+          | and e₁ e₂ ih₁ ih₂ => sorry
+          | _ => sorry
+  end AExp
+
+  namespace Division
+    inductive Arith: Type where
+      | num (n: Nat): Arith
+      | plus (e₁ e₂: Arith): Arith
+      | minus (e₁ e₂: Arith): Arith
+      | mult (e₁ e₂: Arith): Arith
+      | div (e₁ e₂: Arith): Arith
+
+    inductive ArithEval: Arith → Nat → Prop where
+      | num (n: Nat): ArithEval (.num n) n
+      | plus (e₁ e₂: Arith) (n₁ n₂: Nat) (h₁: ArithEval e₁ n₁) (h₂: ArithEval e₂ n₂): ArithEval (.plus e₁ e₂) (n₁ + n₂)
+      | minus (e₁ e₂: Arith) (n₁ n₂: Nat) (h₁: ArithEval e₁ n₁) (h₂: ArithEval e₂ n₂): ArithEval (.minus e₁ e₂) (n₁ - n₂)
+      | mult (e₁ e₂: Arith) (n₁ n₂: Nat) (h₁: ArithEval e₁ n₁) (h₂: ArithEval e₂ n₂): ArithEval (.mult e₁ e₂) (n₁ * n₂)
+      | div (e₁ e₂: Arith) (n₁ n₂ n₃: Nat) (nonZero: n₂ ≠ 0) (prod: n₂ * n₃ = n₁) (h₁: ArithEval e₁ n₁) (h₂: ArithEval e₂ n₂): ArithEval (.div e₁ e₂) n₃
+  end Division
+
+  namespace Any
+    inductive Arith: Type where
+      | any: Arith
+      | num (n: Nat): Arith
+      | plus (e₁ e₂: Arith): Arith
+      | minus (e₁ e₂: Arith): Arith
+      | mult (e₁ e₂: Arith): Arith
+
+    inductive ArithEval: Arith → Nat → Prop where
+      | any (n: Nat): ArithEval .any n
+      | num (n: Nat): ArithEval (.num n) n
+      | plus (e₁ e₂: Arith) (n₁ n₂: Nat) (h₁: ArithEval e₁ n₁) (h₂: ArithEval e₂ n₂): ArithEval (.plus e₁ e₂) (n₁ + n₂)
+      | minus (e₁ e₂: Arith) (n₁ n₂: Nat) (h₁: ArithEval e₁ n₁) (h₂: ArithEval e₂ n₂): ArithEval (.minus e₁ e₂) (n₁ - n₂)
+      | mult (e₁ e₂: Arith) (n₁ n₂: Nat) (h₁: ArithEval e₁ n₁) (h₂: ArithEval e₂ n₂): ArithEval (.mult e₁ e₂) (n₁ * n₂)
+  end Any
+
+  /-
+  ## Expressions with Variables
+  -/
+
+  def State: Type := Maps.TotalMap Nat
+
+  def State.empty: State := Maps.TotalMap.empty 0
+
+  @[reducible]
+  def State.build (l: List (String × Nat)): State :=
+    fold State.empty l
+    where
+      fold (s: State): List (String × Nat) → State
+        | [] => s
+        | (k, v) :: tl => fold (s.update k v) tl
+
   inductive Arith: Type where
     | num (n: Nat): Arith
+    | ident (id: String): Arith
     | plus (e₁ e₂: Arith): Arith
     | minus (e₁ e₂: Arith): Arith
     | mult (e₁ e₂: Arith): Arith
-
-  @[reducible]
-  def Arith.eval: Arith → Nat
-    | .num n => n
-    | .plus e₁ e₂ => e₁.eval + e₂.eval
-    | .minus e₁ e₂ => e₁.eval - e₂.eval
-    | .mult e₁ e₂ => e₁.eval * e₂.eval
-
-  @[reducible]
-  def Arith.optZeroPlus: Arith → Arith
-    | .num n => .num n
-    | .plus (.num 0) e₂ => e₂.optZeroPlus
-    | .plus e₁ e₂ => .plus e₁.optZeroPlus e₂.optZeroPlus
-    | .minus e₁ e₂ => .minus e₁.optZeroPlus e₂.optZeroPlus
-    | .mult e₁ e₂ => .mult e₁.optZeroPlus e₂.optZeroPlus
-
-  example: (Arith.plus (.num 2) (.num 2)).eval = 4 := rfl
-  example: (Arith.plus (.num 2) (.plus (.num 0) (.plus (.num 0) (.num 1)))).optZeroPlus = .plus (.num 2) (.num 1) := rfl
-
-  theorem Arith.optZeroPlus.sound (a: Arith): a.optZeroPlus.eval = a.eval := by
-    induction a with
-      | num n => rfl
-      | plus e₁ e₂ ih₁ ih₂ =>
-        cases e₁ with
-          | num n =>
-            cases n with
-              | zero => simp_all
-              | succ n =>
-                unfold optZeroPlus eval
-                simp_all
-          | plus | minus | mult =>
-            unfold optZeroPlus eval
-            simp_all
-      | minus _ _ ih₁ ih₂ | mult _ _ ih₁ ih₂ =>
-        unfold optZeroPlus eval
-        simp_all
+  deriving DecidableEq
 
   inductive Logic: Type where
     | true: Logic
@@ -66,679 +617,399 @@ namespace AExp
     | gt (e₁ e₂: Arith): Logic
     | not (e: Logic): Logic
     | and (e₁ e₂: Logic): Logic
+  deriving DecidableEq
+
+  /-
+  ### Notations
+  -/
+
+  -- TODO: Implement syntax extensions (https://leanprover.github.io/lean4/doc/macro_overview.html)
+
+  instance: Coe Bool Logic where
+    coe: Bool → Logic
+      | true => Logic.true
+      | false => Logic.false
+  instance: Coe Nat Arith where
+    coe n := Arith.num n
+  instance: OfNat Arith n where
+    ofNat := Arith.num n
+  instance: Coe String Arith where
+    coe id := Arith.ident id
+
+  instance: Add Arith where
+    add x y := Arith.plus x y
+  instance: Sub Arith where
+    sub x y := Arith.minus x y
+  instance: Mul Arith where
+    mul x y := Arith.mult x y
+
+  instance: Neg Logic where
+    neg x := Logic.not x
+
+  /-
+  ### Evaluation
+  -/
 
   @[reducible]
-  def Logic.eval: Logic → Bool
-    | .true => Bool.true
-    | .false => Bool.false
-    | .eq e₁ e₂ => e₁.eval == e₂.eval
-    | .neq e₁ e₂ => e₁.eval != e₂.eval
-    | .le e₁ e₂ => e₁.eval ≤ e₂.eval
-    | .gt e₁ e₂ => e₁.eval > e₂.eval
-    | .not e => !e.eval
-    | .and e₁ e₂ => e₁.eval && e₂.eval
+  def Arith.eval (state: State): Arith → Nat
+    | num n => n
+    | ident id => state id
+    | plus e₁ e₂ => (e₁.eval state) + (e₂.eval state)
+    | minus e₁ e₂ => (e₁.eval state) - (e₂.eval state)
+    | mult e₁ e₂ => (e₁.eval state) * (e₂.eval state)
 
   @[reducible]
-  def Logic.optZeroPlus: Logic → Logic
-    | .true => .true
-    | .false => .false
-    | .eq e₁ e₂ => .eq e₁.optZeroPlus e₂.optZeroPlus
-    | .neq e₁ e₂ => .neq e₁.optZeroPlus e₂.optZeroPlus
-    | .le e₁ e₂ => .le e₁.optZeroPlus e₂.optZeroPlus
-    | .gt e₁ e₂ => .gt e₁.optZeroPlus e₂.optZeroPlus
-    | .not e => .not e.optZeroPlus
-    | .and e₁ e₂ => .and e₁.optZeroPlus e₂.optZeroPlus
+  def Logic.eval (state: State): Logic → Bool
+    | true => Bool.true
+    | false => Bool.false
+    | eq e₁ e₂ => (e₁.eval state) == (e₂.eval state)
+    | neq e₁ e₂ => (e₁.eval state) != (e₂.eval state)
+    | le e₁ e₂ => (e₁.eval state) ≤ (e₂.eval state)
+    | gt e₁ e₂ => (e₁.eval state) > (e₂.eval state)
+    | not e => !(e.eval state)
+    | and e₁ e₂ => (e₁.eval state) && (e₂.eval state)
+
+  example: ((3: Arith) + "X" * 2).eval (State.build [("X", 5)]) = 13 := rfl
+  example: (("Z": Arith) + "X" * "Y").eval (State.build [("X", 5), ("Y", 4)]) = 20 := rfl
+  example: (Logic.and true (.not (.le "X" 4))).eval (State.build [("X", 5)]) = true := rfl
 
   /-
-  ## Lean (Coq) Automation
+  ## Commands
   -/
 
-  /-
-  ### The `try` Tactical
-  -/
-
-  example (P: Prop) (h: P): P := by
-    try rfl
-    apply h
-
-  example (a: Arith): a.eval = a.eval := by
-    try rfl
-
-  /-
-  ### The `<;>` Tactical (Simple Form)
-  -/
-
-  example (n: Nat): 0 ≤ n := by
-    cases n with
-      | zero => simp
-      | succ n => simp
-
-  example (n: Nat): 0 ≤ n := by
-    cases n <;> simp
-
-  /-
-  ### The `<;>` Tactical (General Form)
-  -/
-
-  example (a: Arith): a.optZeroPlus.eval = a.eval := by
-    induction a <;>
-    try (first | rfl
-               | unfold Arith.optZeroPlus Arith.eval
-                 simp_all)
-    case plus e₁ _ ih₁ ih₂ =>
-      cases e₁ <;>
-      try (unfold Arith.optZeroPlus Arith.eval
-           rw [ih₁, ih₂])
-      case num n =>
-        cases n with
-          | zero => simp_all
-          | succ n =>
-            unfold Arith.optZeroPlus Arith.eval
-            simp_all
-
-  /-
-  ### The `repeat` Tactical
-  -/
-
-  def In (x: α) (l: List α): Prop :=
-    match l with
-      | [] => False
-      | b :: m => b = x \/ In x m
-
-  example: In 10 [1, 2, 3, 4, 5, 6, 7, 8, 9, 10] := by
-    repeat (try (first | apply Or.inl; rfl | apply Or.inr))
-
-  theorem Logic.optZeroPlus.sound (e: Logic): e.optZeroPlus.eval = e.eval := by
-    induction e <;>
-    try (first | rfl
-               | unfold Logic.optZeroPlus Logic.eval
-                 simp [Arith.optZeroPlus.sound])
-    case not e ih =>
-      unfold Logic.optZeroPlus Logic.eval
-      rw [ih]
-    case and e₁ e₂ ih₁ ih₂ =>
-      unfold Logic.optZeroPlus Logic.eval
-      rw [ih₁, ih₂]
-
-  -- TODO: Moar optimization
-
-  /-
-  ## Defining New Tactics
-  -/
-
-  -- TODO: Research defining tactics in Lean
-
-  /-
-  ## The `linearith` (`lia`) Tactic
-  -/
-
-  -- import Mathlib.tactics.linarith
-
-  example (n₁ n₂ n₃ n₄: Nat) (h: n₁ + n₂ ≤ n₂ + n₃ ∧ n₃ + 3 = n₄ + 3): n₁ ≤ n₄ := by
-    linarith
-
-  example (n₁ n₂: Nat): n₁ + n₂ = n₂ + n₁ := by
-    linarith
-
-  example (n₁ n₂ n₃: Nat): n₁ + (n₂ + n₃) = (n₁ + n₂) + n₃ := by
-    linarith
-
-  /-
-  ## A Few More Handy Tactics
-  -/
-
-  -- TODO: Research the same tactics in Lean
-
-  /-
-  ## Evaluation as a Relation
-  -/
-
-  inductive ArithEval: Arith → Nat → Prop where
-    | num (n: Nat): ArithEval (.num n) n
-    | plus (e₁ e₂: Arith) (n₁ n₂: Nat) (h₁: ArithEval e₁ n₁) (h₂: ArithEval e₂ n₂): ArithEval (.plus e₁ e₂) (n₁ + n₂)
-    | minus (e₁ e₂: Arith) (n₁ n₂: Nat) (h₁: ArithEval e₁ n₁) (h₂: ArithEval e₂ n₂): ArithEval (.minus e₁ e₂) (n₁ - n₂)
-    | mult (e₁ e₂: Arith) (n₁ n₂: Nat) (h₁: ArithEval e₁ n₁) (h₂: ArithEval e₂ n₂): ArithEval (.mult e₁ e₂) (n₁ * n₂)
-
-  /-
-  ### Inference Rule Notation
-  -/
-
-  inductive LogicEval: Logic → Bool → Prop where
-    | true: LogicEval .true true
-    | false: LogicEval .false false
-    | eq (e₁ e₂: Arith) (n₁ n₂: Nat) (h₁: ArithEval e₁ n₁) (h₂: ArithEval e₂ n₂): LogicEval (.eq e₁ e₂) (n₁ == n₂)
-    | neq (e₁ e₂: Arith) (n₁ n₂: Nat) (h₁: ArithEval e₁ n₁) (h₂: ArithEval e₂ n₂): LogicEval (.neq e₁ e₂) (n₁ != n₂)
-    | le (e₁ e₂: Arith) (n₁ n₂: Nat) (h₁: ArithEval e₁ n₁) (h₂: ArithEval e₂ n₂): LogicEval (.neq e₁ e₂) (n₁ ≤ n₂)
-    | gt (e₁ e₂: Arith) (n₁ n₂: Nat) (h₁: ArithEval e₁ n₁) (h₂: ArithEval e₂ n₂): LogicEval (.neq e₁ e₂) (n₁ > n₂)
-    | not (e: Logic) (b: Bool) (h: LogicEval e b): LogicEval (.not e) !b
-    | and (e₁ e₂: Logic) (b₁ b₂: Bool) (h₁: LogicEval e₁ b₁) (h₂: LogicEval e₂ b₂): LogicEval (.and e₁ e₂) (b₁ && b₂)
-
-  /-
-  ### Equivalence of Definitions
-  -/
-
-  theorem arith_eval_eval (a: Arith) (n: Nat): ArithEval a n ↔ a.eval = n := by
-    apply Iff.intro
-    · intro h
-      induction h <;> first | rfl
-                            | unfold Arith.eval
-                              simp_all
-    · intro h₁
-      induction a with
-        | num n =>
-          rw [← h₁]
-          exact ArithEval.num n
-        | plus e₁ e₂ ih₁ ih₂ =>
-          unfold Arith.eval at h₁
-          sorry
-        | _ => sorry
-
-  theorem logic_eval_eval (l: Logic) (b: Bool): LogicEval l b ↔ l.eval = b := by
-    apply Iff.intro
-    · intro h
-      induction h with
-        | true => rfl
-        | false => rfl
-        | eq e₁ e₂ n₁ n₂ h₁ h₂ =>
-          unfold Logic.eval
-          rw [arith_eval_eval] at *
-          simp_all
-        | neq e₁ e₂ n₁ n₂ h₁ h₂ =>
-          unfold Logic.eval
-          rw [arith_eval_eval] at *
-          simp_all
-        | le e₁ e₂ n₁ n₂ h₁ h₂ =>
-          unfold Logic.eval
-          rw [arith_eval_eval] at *
-          simp_all
-          sorry
-        | gt e₁ e₂ n₁ n₂ h₁ h₂ =>
-          unfold Logic.eval
-          rw [arith_eval_eval] at *
-          simp_all
-          sorry
-        | not e b h ih =>
-          unfold Logic.eval
-          rw [ih]
-        | and e₁ e₂ b₁ b₂ h₁ h₂ ih₁ ih₂ =>
-          unfold Logic.eval
-          rw [ih₁, ih₂]
-    · intro h
-      induction l with
-        | true =>
-          cases b with
-            | true => exact LogicEval.true
-            | false => contradiction
-        | false =>
-          cases b with
-            | true => contradiction
-            | false => exact LogicEval.false
-        | eq e₁ e₂ =>
-          unfold Logic.eval at h
-          sorry
-        -- Other Arith cases
-        | not e ih => sorry
-        | and e₁ e₂ ih₁ ih₂ => sorry
-        | _ => sorry
-end AExp
-
-namespace Division
-  inductive Arith: Type where
-    | num (n: Nat): Arith
-    | plus (e₁ e₂: Arith): Arith
-    | minus (e₁ e₂: Arith): Arith
-    | mult (e₁ e₂: Arith): Arith
-    | div (e₁ e₂: Arith): Arith
-
-  inductive ArithEval: Arith → Nat → Prop where
-    | num (n: Nat): ArithEval (.num n) n
-    | plus (e₁ e₂: Arith) (n₁ n₂: Nat) (h₁: ArithEval e₁ n₁) (h₂: ArithEval e₂ n₂): ArithEval (.plus e₁ e₂) (n₁ + n₂)
-    | minus (e₁ e₂: Arith) (n₁ n₂: Nat) (h₁: ArithEval e₁ n₁) (h₂: ArithEval e₂ n₂): ArithEval (.minus e₁ e₂) (n₁ - n₂)
-    | mult (e₁ e₂: Arith) (n₁ n₂: Nat) (h₁: ArithEval e₁ n₁) (h₂: ArithEval e₂ n₂): ArithEval (.mult e₁ e₂) (n₁ * n₂)
-    | div (e₁ e₂: Arith) (n₁ n₂ n₃: Nat) (nonZero: n₂ ≠ 0) (prod: n₂ * n₃ = n₁) (h₁: ArithEval e₁ n₁) (h₂: ArithEval e₂ n₂): ArithEval (.div e₁ e₂) n₃
-end Division
-
-namespace Any
-  inductive Arith: Type where
-    | any: Arith
-    | num (n: Nat): Arith
-    | plus (e₁ e₂: Arith): Arith
-    | minus (e₁ e₂: Arith): Arith
-    | mult (e₁ e₂: Arith): Arith
-
-  inductive ArithEval: Arith → Nat → Prop where
-    | any (n: Nat): ArithEval .any n
-    | num (n: Nat): ArithEval (.num n) n
-    | plus (e₁ e₂: Arith) (n₁ n₂: Nat) (h₁: ArithEval e₁ n₁) (h₂: ArithEval e₂ n₂): ArithEval (.plus e₁ e₂) (n₁ + n₂)
-    | minus (e₁ e₂: Arith) (n₁ n₂: Nat) (h₁: ArithEval e₁ n₁) (h₂: ArithEval e₂ n₂): ArithEval (.minus e₁ e₂) (n₁ - n₂)
-    | mult (e₁ e₂: Arith) (n₁ n₂: Nat) (h₁: ArithEval e₁ n₁) (h₂: ArithEval e₂ n₂): ArithEval (.mult e₁ e₂) (n₁ * n₂)
-end Any
-
-/-
-## Expressions with Variables
--/
-
-def State: Type := TotalMap Nat
-
-def State.empty: State := TotalMap.empty 0
-
-@[reducible]
-def State.build (l: List (String × Nat)): State :=
-  fold State.empty l
-  where
-    fold (s: State): List (String × Nat) → State
-      | [] => s
-      | (k, v) :: tl => fold (s.update k v) tl
-
-inductive Arith: Type where
-  | num (n: Nat): Arith
-  | ident (id: String): Arith
-  | plus (e₁ e₂: Arith): Arith
-  | minus (e₁ e₂: Arith): Arith
-  | mult (e₁ e₂: Arith): Arith
-deriving DecidableEq
-
-inductive Logic: Type where
-  | true: Logic
-  | false: Logic
-  | eq (e₁ e₂: Arith): Logic
-  | neq (e₁ e₂: Arith): Logic
-  | le (e₁ e₂: Arith): Logic
-  | gt (e₁ e₂: Arith): Logic
-  | not (e: Logic): Logic
-  | and (e₁ e₂: Logic): Logic
-deriving DecidableEq
-
-/-
-### Notations
--/
-
--- TODO: Implement syntax extensions (https://leanprover.github.io/lean4/doc/macro_overview.html)
-
-instance: Coe Bool Logic where
-  coe: Bool → Logic
-    | true => Logic.true
-    | false => Logic.false
-instance: Coe Nat Arith where
-  coe n := Arith.num n
-instance: OfNat Arith n where
-  ofNat := Arith.num n
-instance: Coe String Arith where
-  coe id := Arith.ident id
-
-instance: Add Arith where
-  add x y := Arith.plus x y
-instance: Sub Arith where
-  sub x y := Arith.minus x y
-instance: Mul Arith where
-  mul x y := Arith.mult x y
-
-instance: Neg Logic where
-  neg x := Logic.not x
-
-/-
-### Evaluation
--/
-
-@[reducible]
-def Arith.eval (state: State): Arith → Nat
-  | num n => n
-  | ident id => state id
-  | plus e₁ e₂ => (e₁.eval state) + (e₂.eval state)
-  | minus e₁ e₂ => (e₁.eval state) - (e₂.eval state)
-  | mult e₁ e₂ => (e₁.eval state) * (e₂.eval state)
-
-@[reducible]
-def Logic.eval (state: State): Logic → Bool
-  | true => Bool.true
-  | false => Bool.false
-  | eq e₁ e₂ => (e₁.eval state) == (e₂.eval state)
-  | neq e₁ e₂ => (e₁.eval state) != (e₂.eval state)
-  | le e₁ e₂ => (e₁.eval state) ≤ (e₂.eval state)
-  | gt e₁ e₂ => (e₁.eval state) > (e₂.eval state)
-  | not e => !(e.eval state)
-  | and e₁ e₂ => (e₁.eval state) && (e₂.eval state)
-
-example: ((3: Arith) + "X" * 2).eval (State.build [("X", 5)]) = 13 := rfl
-example: (("Z": Arith) + "X" * "Y").eval (State.build [("X", 5), ("Y", 4)]) = 20 := rfl
-example: (Logic.and true (.not (.le "X" 4))).eval (State.build [("X", 5)]) = true := rfl
-
-/-
-## Commands
--/
-
-inductive Command: Type where
-  | skip: Command
-  | assign (id: String) (e: Arith): Command
-  | seq (c₁ c₂: Command): Command
-  | if (b: Logic) (c₁ c₂: Command): Command
-  | while (b: Logic) (c: Command): Command
-
-instance: Coe (List Command) Command where
-  coe l :=
-    let rec conv: List Command → Command
-      | [] => .skip
-      | hd::[] => hd
-      | hd::tl => .seq hd (conv tl)
-    conv l
-
-def factorial: Command :=
-  [
-    (Command.assign "Z" "X"),
-    (.assign "Y" 1),
-    (.while (.neq "Z" 0) [
-      (Command.assign "Y" ("Y" * "Z")),
-      (.assign "Z" ("Z" - 1))
-    ])
-  ]
-
-/-
-### Desugaring Notations
--/
-
-set_option pp.notation true
-set_option pp.coercions false
-
-#print factorial
-
-set_option pp.notation false
-set_option pp.coercions true
-
-/-
-### Locate, Again
--/
-
--- Appears to be Coq specific
-
-/- #### Finding Identifiers -/
-/- #### Finding Notations -/
-
-/-
-### More Examples
--/
-
-section
-  /- #### Assignment -/
-
-  def plus2: Command := .assign "X" ("X" + 2)
-  def xTimesYInZ: Command := .assign "Z" ("X" * "Y")
-
-  /- #### Loops -/
-
-  private def subtractSlowlyBody: Command := ([
-    (.assign "Z" ("Z" - 1)),
-    (.assign "X" ("X" - 1))
-  ]: List Command)
-
-  private def subtractSlowly: Command :=
-    .while (.neq "X" 0) subtractSlowlyBody
-
-  private def subtract3From5Slowly: Command := ([
-    (.assign "X" 3),
-    (.assign "Z" 5),
-    subtractSlowly
-  ]: List Command)
-
-  /- #### An Infinite Loop -/
-
-  def loopForever: Command := .while .true .skip
-end
-
-/-
-## Evaluating Commands
--/
-
-def Command.noBueno (state: State): Command → State
-  | .skip => state
-  | .assign id e => state.update id (e.eval state)
-  | .seq c₁ c₂ =>
-    state
-      |> c₁.noBueno
-      |> c₂.noBueno
-  | .if c t f =>
-    if c.eval state
-    then t.noBueno state
-    else f.noBueno state
-  | .while _ _ => state
-
-/-
-### Evaluation as a Relation
--/
-
-inductive CommandEval: Command → State → State → Prop where
-  | skip (s: State): CommandEval .skip s s
-  | assign {e: Arith} {n: Nat} {id: String} (s: State) (h: e.eval s = n): CommandEval (.assign id e) s (s.update id n)
-  | seq {c₁ c₂: Command} (s₁ s₂ s₃: State) (h₁: CommandEval c₁ s₁ s₂) (h₂: CommandEval c₂ s₂ s₃): CommandEval (.seq c₁ c₂) s₁ s₃
-  | ifTrue {c: Logic} {t f: Command} (s₁ s₂: State) (h₁: c.eval s₁ = .true) (h₂: CommandEval t s₁ s₂): CommandEval (.if c t f) s₁ s₂
-  | ifFalse {c: Logic} {t f: Command} (s₁ s₂: State) (h₁: c.eval s₁ = .false) (h₂: CommandEval f s₁ s₂): CommandEval (.if c t f) s₁ s₂
-  | whileTrue {c: Logic} {b: Command} (s₁ s₂ s₃: State) (h₁: c.eval s₁ = .true) (h₂: CommandEval b s₁ s₂) (h₃: CommandEval (.while c b) s₂ s₃): CommandEval (.while c b) s₁ s₃
-  | whileFalse {c: Logic} {b: Command} (s: State) (h₁: c.eval s = .false): CommandEval (.while c b) s s
-
-def assignment (id: String) (n: Nat) (s: State): CommandEval (Command.assign id (n: Arith)) s (s.update id n) :=
-    have h: (n: Arith).eval s = n := by
-      unfold Arith.eval
-      rfl
-    CommandEval.assign s h
-
-section
-  /- Useful definitions to save typing -/
-
-  private def x0: Command := .assign "X" 0
-  private def x2: Command := .assign "X" 2
-  private def y1: Command := .assign "Y" 1
-  private def y3: Command := .assign "Y" 3
-  private def z2: Command := .assign "Z" 2
-  private def z4: Command := .assign "Z" 4
-
-  private def xLe1: Logic := .le "X" 1
-
-  private def branch: Command := Command.if xLe1 y3 z4
-
-  /- Example -/
-
-  /- x := 2; if x ≤ 1 then y := 3 else z := 4 -/
-  example: CommandEval [x2, branch] State.empty (State.build [("X", 2), ("Z", 4)]) :=
-    let s₁: State := State.empty
-    let s₂: State := s₁.update "X" 2
-    let s₃: State := s₂.update "Z" 4
-
-    have h₁: CommandEval x2 s₁ s₂ := assignment "X" 2 s₁
-    have h₂: CommandEval branch s₂ s₃ :=
-      have h₁: (Logic.le "X" 1).eval s₂ = false := by
-        unfold Logic.eval
-        rfl
-      have h₂: CommandEval z4 s₂ s₃ := assignment "Z" 4 s₂
-      CommandEval.ifFalse s₂ s₃ h₁ h₂
-
-    by
-      repeat unfold instCoeListCommand.conv
-      exact CommandEval.seq s₁ s₂ s₃ h₁ h₂
-
-  /- x := 0; y := 1; z := 2 -/
-  example: CommandEval [x0, y1, z2] State.empty (State.build [("X", 0), ("Y", 1), ("Z", 2)]) :=
-    let s₁: State := State.empty
-    let s₂: State := s₁.update "X" 0
-    let s₃: State := s₂.update "Y" 1
-    let s₄: State := s₃.update "Z" 2
-
-    by
-      repeat unfold instCoeListCommand.conv
-      sorry
-
-  def sum: Command :=
-    Command.seq
-      (.assign "Y" 0)
-      (.while (.gt "X" 0)
-        (.seq (.assign "Y" ("X" + "Y"))
-              (.assign "X" ("X" - 1))))
-
-  example: CommandEval sum (State.build [("X", 2)]) (State.build [("X", 2), ("Y", 0), ("Y", 2), ("X", 1), ("Y", 3), ("X", 0)]) :=
-    sorry
-end
-
-/-
-### Determinism of Evaluation
--/
-
-theorem CommandEval.deterministic (c: Command) (s₁ s₂ s₃: State) (h₁: CommandEval c s₁ s₂) (h₂: CommandEval c s₁ s₃): s₂ = s₃ := by
-  sorry
-
-/-
-## Reasoning about Imp Programs
--/
-
-example (s₁ s₂: State) (n: Nat) (h₁: s₁ "X" = n) (h₂: CommandEval plus2 s₁ s₂): s₂ "X" = n + 2 := by
-  cases h₂ with
-    | assign _ h =>
-      simp
-      repeat unfold Arith.eval at h
-      rw [h₁] at h
-      apply Eq.symm
-      exact h
-
-example (s₁ s₂: State) (n₁ n₂: Nat) (h₁: s₁ "X" = n₁) (h₂: s₁ "Y" = n₂) (h₃: CommandEval xTimesYInZ s₁ s₂): s₂ "Z" = n₁ * n₂ := by
-  cases h₃ with
-    | assign _ h =>
-      repeat unfold Arith.eval at h
-      repeat unfold Arith.eval at h
-      rw [h₁, h₂] at h
-      simp_all
-
-example (s₁ s₂: State): ¬CommandEval loopForever s₁ s₂ := by
-  unfold Not
-  intro h
-  unfold loopForever at h
-  cases h with
-    | whileTrue h₁ h₂ h₃ => sorry
-    | whileFalse h₁ => contradiction
-
-def Command.noWhiles: Command → Bool
-  | .skip | .assign _ _ | .seq _ _ | .if _ _ _ => true
-  | _ => false
-
-inductive NoWhiles: Command → Prop where
-  | skip: NoWhiles .skip
-  | assign {id: String} {e: Arith}: NoWhiles (.assign id e)
-  | seq {c₁ c₂: Command}: NoWhiles (.seq c₁ c₂)
-  | if {c: Logic} {t f: Command}: NoWhiles (.if c t f)
-
-theorem NoWhiles.noWhiles (c: Command): c.noWhiles = true ↔ NoWhiles c := by
-  sorry
-
-theorem CommandEval.noWhiles_terminate (s₁ s₂: State) (c: Command) (h: NoWhiles c): CommandEval c s₁ s₂ := by
-  sorry
-
-/-
-## Additional Exercises
--/
-
-abbrev Stack: Type := List Nat
-
-def Stack.empty: Stack := []
-
-inductive StackInstr: Type where
-  | push (n: Nat): StackInstr
-  | load (id: String): StackInstr
-  | plus: StackInstr
-  | minus: StackInstr
-  | mult: StackInstr
-
-@[reducible]
-def StackInstr.eval (state: State): StackInstr → Stack → Stack
-  | .push n, stack => n :: stack
-  | .load id, stack => (state id) :: stack
-  | .plus, r :: l :: stack => (l + r) :: stack
-  | .minus, r :: l :: stack => (l - r) :: stack
-  | .mult, r :: l :: stack => (l * r) :: stack
-  | _, stack => stack
-
-abbrev Program: Type := List StackInstr
-
-@[reducible]
-def Program.eval (state: State) (program: Program) (init: Stack): Stack :=
-  program.foldl (fun stack instr => instr.eval state stack) init
-
-example: Program.eval State.empty [StackInstr.push 5, .push 3, .push 1, .minus] Stack.empty = [2, 5] := by rfl
-example: Program.eval (State.build [("X", 3)]) [StackInstr.push 4, .load "X", .mult, .plus] [3, 4] = [15, 4] := rfl
-
-@[reducible]
-def Arith.compile: Arith → Program
-  | .num n => [.push n]
-  | .ident id => [.load id]
-  | .plus e₁ e₂ => e₁.compile ++ e₂.compile ++ [.plus]
-  | .minus e₁ e₂ => e₁.compile ++ e₂.compile ++ [.minus]
-  | .mult e₁ e₂ => e₁.compile ++ e₂.compile ++ [.mult]
-
-example: (Arith.minus "X" (.mult 2 "Y")).compile = [StackInstr.load "X", .push 2, .load "Y", .mult, .minus] := rfl
-
-theorem eval_append (state: State) (p₁ p₂: Program) (stack: Stack): (p₁ ++ p₂).eval state stack = p₂.eval state (p₁.eval state stack) := by
-  sorry
-
-theorem Arith.compile.correct (state: State) (e: Arith): e.compile.eval state Stack.empty = [e.eval state] := by
-  sorry
-  where
-  helper (state: State) (stack: Stack) (e: Arith): e.compile.eval state stack = e.eval state :: stack := by
-    sorry
-
-@[reducible]
-def Logic.shortCircuitEval (state: State): Logic → Bool
-  | .and e₁ e₂ =>
-    if e₁.eval state
-    then Bool.true
-    else e₂.eval state
-  | l => l.eval state
-
-theorem Logic.shortCircuitEval.eval (state: State) (b: Logic): b.shortCircuitEval state = b.eval state := by
-  induction b
-  <;> try rfl
-  case and e₁ e₂ h₁ h₂ =>
-    sorry
-
-namespace BreakImp
   inductive Command: Type where
     | skip: Command
-    | break: Command
     | assign (id: String) (e: Arith): Command
     | seq (c₁ c₂: Command): Command
     | if (b: Logic) (c₁ c₂: Command): Command
     | while (b: Logic) (c: Command): Command
 
-  inductive Result: Type where
-    | continue: Result
-    | break: Result
+  instance: Coe (List Command) Command where
+    coe l :=
+      let rec conv: List Command → Command
+        | [] => .skip
+        | hd::[] => hd
+        | hd::tl => .seq hd (conv tl)
+      conv l
 
-  inductive CommandEval: Command → State → Result → State → Prop where
-    | skip (s: State): CommandEval .skip s .continue s
-    | break (s: State): CommandEval .break s .break s
-    | assign {e: Arith} {n: Nat} {id: String} (s: State) (h: e.eval s = n): CommandEval (.assign id e) s .continue (s.update id n)
-    | seq {c₁ c₂: Command} (s₁ s₂ s₃: State) (h₁: CommandEval c₁ s₁ .continue s₂) (h₂: CommandEval c₂ s₂ .continue s₃): CommandEval (.seq c₁ c₂) s₁ .continue s₃
-    | ifTrue {c: Logic} {t f: Command} (s₁ s₂: State) (h₁: c.eval s₁ = .true) (h₂: CommandEval t s₁ .continue s₂): CommandEval (.if c t f) s₁ .continue s₂
-    | ifFalse {c: Logic} {t f: Command} (s₁ s₂: State) (h₁: c.eval s₁ = .false) (h₂: CommandEval f s₁ .continue s₂): CommandEval (.if c t f) s₁ .continue s₂
-    | whileTrue {c: Logic} {b: Command} (s₁ s₂ s₃: State) (h₁: c.eval s₁ = .true) (h₂: CommandEval b s₁ .continue s₂) (h₃: CommandEval (.while c b) s₂ .continue s₃): CommandEval (.while c b) s₁ .continue s₃
-    | whileFalse {c: Logic} {b: Command} (s: State) (h₁: c.eval s = .false): CommandEval (.while c b) s .continue s
+  def factorial: Command :=
+    [
+      (Command.assign "Z" "X"),
+      (.assign "Y" 1),
+      (.while (.neq "Z" 0) [
+        (Command.assign "Y" ("Y" * "Z")),
+        (.assign "Z" ("Z" - 1))
+      ])
+    ]
 
-  example (c: Command) (s₁ s₂: State) (r: Result): CommandEval (.seq .break c) s₁ r s₂ := by
+  /-
+  ### Desugaring Notations
+  -/
+
+  set_option pp.notation true
+  set_option pp.coercions false
+
+  #print factorial
+
+  set_option pp.notation false
+  set_option pp.coercions true
+
+  /-
+  ### Locate, Again
+  -/
+
+  -- Appears to be Coq specific
+
+  /- #### Finding Identifiers -/
+  /- #### Finding Notations -/
+
+  /-
+  ### More Examples
+  -/
+
+  section
+    /- #### Assignment -/
+
+    def plus2: Command := .assign "X" ("X" + 2)
+    def xTimesYInZ: Command := .assign "Z" ("X" * "Y")
+
+    /- #### Loops -/
+
+    private def subtractSlowlyBody: Command := ([
+      (.assign "Z" ("Z" - 1)),
+      (.assign "X" ("X" - 1))
+    ]: List Command)
+
+    private def subtractSlowly: Command :=
+      .while (.neq "X" 0) subtractSlowlyBody
+
+    private def subtract3From5Slowly: Command := ([
+      (.assign "X" 3),
+      (.assign "Z" 5),
+      subtractSlowly
+    ]: List Command)
+
+    /- #### An Infinite Loop -/
+
+    def loopForever: Command := .while .true .skip
+  end
+
+  /-
+  ## Evaluating Commands
+  -/
+
+  def Command.noBueno (state: State): Command → State
+    | .skip => state
+    | .assign id e => state.update id (e.eval state)
+    | .seq c₁ c₂ =>
+      state
+        |> c₁.noBueno
+        |> c₂.noBueno
+    | .if c t f =>
+      if c.eval state
+      then t.noBueno state
+      else f.noBueno state
+    | .while _ _ => state
+
+  /-
+  ### Evaluation as a Relation
+  -/
+
+  inductive CommandEval: Command → State → State → Prop where
+    | skip (s: State): CommandEval .skip s s
+    | assign {e: Arith} {n: Nat} {id: String} (s: State) (h: e.eval s = n): CommandEval (.assign id e) s (s.update id n)
+    | seq {c₁ c₂: Command} (s₁ s₂ s₃: State) (h₁: CommandEval c₁ s₁ s₂) (h₂: CommandEval c₂ s₂ s₃): CommandEval (.seq c₁ c₂) s₁ s₃
+    | ifTrue {c: Logic} {t f: Command} (s₁ s₂: State) (h₁: c.eval s₁ = .true) (h₂: CommandEval t s₁ s₂): CommandEval (.if c t f) s₁ s₂
+    | ifFalse {c: Logic} {t f: Command} (s₁ s₂: State) (h₁: c.eval s₁ = .false) (h₂: CommandEval f s₁ s₂): CommandEval (.if c t f) s₁ s₂
+    | whileTrue {c: Logic} {b: Command} (s₁ s₂ s₃: State) (h₁: c.eval s₁ = .true) (h₂: CommandEval b s₁ s₂) (h₃: CommandEval (.while c b) s₂ s₃): CommandEval (.while c b) s₁ s₃
+    | whileFalse {c: Logic} {b: Command} (s: State) (h₁: c.eval s = .false): CommandEval (.while c b) s s
+
+  def assignment (id: String) (n: Nat) (s: State): CommandEval (Command.assign id (n: Arith)) s (s.update id n) :=
+      have h: (n: Arith).eval s = n := by
+        unfold Arith.eval
+        rfl
+      CommandEval.assign s h
+
+  section
+    /- Useful definitions to save typing -/
+
+    private def x0: Command := .assign "X" 0
+    private def x2: Command := .assign "X" 2
+    private def y1: Command := .assign "Y" 1
+    private def y3: Command := .assign "Y" 3
+    private def z2: Command := .assign "Z" 2
+    private def z4: Command := .assign "Z" 4
+
+    private def xLe1: Logic := .le "X" 1
+
+    private def branch: Command := Command.if xLe1 y3 z4
+
+    /- Example -/
+
+    /- x := 2; if x ≤ 1 then y := 3 else z := 4 -/
+    example: CommandEval [x2, branch] State.empty (State.build [("X", 2), ("Z", 4)]) :=
+      let s₁: State := State.empty
+      let s₂: State := s₁.update "X" 2
+      let s₃: State := s₂.update "Z" 4
+
+      have h₁: CommandEval x2 s₁ s₂ := assignment "X" 2 s₁
+      have h₂: CommandEval branch s₂ s₃ :=
+        have h₁: (Logic.le "X" 1).eval s₂ = false := by
+          unfold Logic.eval
+          rfl
+        have h₂: CommandEval z4 s₂ s₃ := assignment "Z" 4 s₂
+        CommandEval.ifFalse s₂ s₃ h₁ h₂
+
+      by
+        repeat unfold instCoeListCommand.conv
+        exact CommandEval.seq s₁ s₂ s₃ h₁ h₂
+
+    /- x := 0; y := 1; z := 2 -/
+    example: CommandEval [x0, y1, z2] State.empty (State.build [("X", 0), ("Y", 1), ("Z", 2)]) :=
+      let s₁: State := State.empty
+      let s₂: State := s₁.update "X" 0
+      let s₃: State := s₂.update "Y" 1
+      let s₄: State := s₃.update "Z" 2
+
+      by
+        repeat unfold instCoeListCommand.conv
+        sorry
+
+    def sum: Command :=
+      Command.seq
+        (.assign "Y" 0)
+        (.while (.gt "X" 0)
+          (.seq (.assign "Y" ("X" + "Y"))
+                (.assign "X" ("X" - 1))))
+
+    example: CommandEval sum (State.build [("X", 2)]) (State.build [("X", 2), ("Y", 0), ("Y", 2), ("X", 1), ("Y", 3), ("X", 0)]) :=
+      sorry
+  end
+
+  /-
+  ### Determinism of Evaluation
+  -/
+
+  theorem CommandEval.deterministic (c: Command) (s₁ s₂ s₃: State) (h₁: CommandEval c s₁ s₂) (h₂: CommandEval c s₁ s₃): s₂ = s₃ := by
     sorry
 
-  example (c: Logic) (b: Command) (s₁ s₂: State) (r: Result): CommandEval (.while c b) s₁ r s₂ := by
+  /-
+  ## Reasoning about Imp Programs
+  -/
+
+  example (s₁ s₂: State) (n: Nat) (h₁: s₁ "X" = n) (h₂: CommandEval plus2 s₁ s₂): s₂ "X" = n + 2 := by
+    cases h₂ with
+      | assign _ h =>
+        simp
+        repeat unfold Arith.eval at h
+        rw [h₁] at h
+        apply Eq.symm
+        exact h
+
+  example (s₁ s₂: State) (n₁ n₂: Nat) (h₁: s₁ "X" = n₁) (h₂: s₁ "Y" = n₂) (h₃: CommandEval xTimesYInZ s₁ s₂): s₂ "Z" = n₁ * n₂ := by
+    cases h₃ with
+      | assign _ h =>
+        repeat unfold Arith.eval at h
+        repeat unfold Arith.eval at h
+        rw [h₁, h₂] at h
+        simp_all
+
+  example (s₁ s₂: State): ¬CommandEval loopForever s₁ s₂ := by
+    unfold Not
+    intro h
+    unfold loopForever at h
+    cases h with
+      | whileTrue h₁ h₂ h₃ => sorry
+      | whileFalse h₁ => contradiction
+
+  def Command.noWhiles: Command → Bool
+    | .skip | .assign _ _ | .seq _ _ | .if _ _ _ => true
+    | _ => false
+
+  inductive NoWhiles: Command → Prop where
+    | skip: NoWhiles .skip
+    | assign {id: String} {e: Arith}: NoWhiles (.assign id e)
+    | seq {c₁ c₂: Command}: NoWhiles (.seq c₁ c₂)
+    | if {c: Logic} {t f: Command}: NoWhiles (.if c t f)
+
+  theorem NoWhiles.noWhiles (c: Command): c.noWhiles = true ↔ NoWhiles c := by
     sorry
 
-  example (c: Logic) (b: Command) (s₁ s₂: State) (h₁: c.eval s₁ = true) (h₂: CommandEval b s₁ .break s₂): CommandEval (.while c b) s₁ .continue s₂ := by
+  theorem CommandEval.noWhiles_terminate (s₁ s₂: State) (c: Command) (h: NoWhiles c): CommandEval c s₁ s₂ := by
     sorry
 
-  example (c₁ c₂: Command) (s₁ s₂ s₃: State) (h₁: CommandEval c₁ s₁ .continue s₂) (h₂: CommandEval c₂ s₂ .continue s₃): CommandEval (.seq c₁ c₂) s₁ .continue s₂ := by
+  /-
+  ## Additional Exercises
+  -/
+
+  abbrev Stack: Type := List Nat
+
+  def Stack.empty: Stack := []
+
+  inductive StackInstr: Type where
+    | push (n: Nat): StackInstr
+    | load (id: String): StackInstr
+    | plus: StackInstr
+    | minus: StackInstr
+    | mult: StackInstr
+
+  @[reducible]
+  def StackInstr.eval (state: State): StackInstr → Stack → Stack
+    | .push n, stack => n :: stack
+    | .load id, stack => (state id) :: stack
+    | .plus, r :: l :: stack => (l + r) :: stack
+    | .minus, r :: l :: stack => (l - r) :: stack
+    | .mult, r :: l :: stack => (l * r) :: stack
+    | _, stack => stack
+
+  abbrev Program: Type := List StackInstr
+
+  @[reducible]
+  def Program.eval (state: State) (program: Program) (init: Stack): Stack :=
+    program.foldl (fun stack instr => instr.eval state stack) init
+
+  example: Program.eval State.empty [StackInstr.push 5, .push 3, .push 1, .minus] Stack.empty = [2, 5] := by rfl
+  example: Program.eval (State.build [("X", 3)]) [StackInstr.push 4, .load "X", .mult, .plus] [3, 4] = [15, 4] := rfl
+
+  @[reducible]
+  def Arith.compile: Arith → Program
+    | .num n => [.push n]
+    | .ident id => [.load id]
+    | .plus e₁ e₂ => e₁.compile ++ e₂.compile ++ [.plus]
+    | .minus e₁ e₂ => e₁.compile ++ e₂.compile ++ [.minus]
+    | .mult e₁ e₂ => e₁.compile ++ e₂.compile ++ [.mult]
+
+  example: (Arith.minus "X" (.mult 2 "Y")).compile = [StackInstr.load "X", .push 2, .load "Y", .mult, .minus] := rfl
+
+  theorem eval_append (state: State) (p₁ p₂: Program) (stack: Stack): (p₁ ++ p₂).eval state stack = p₂.eval state (p₁.eval state stack) := by
     sorry
 
-  example (c₁ c₂: Command) (s₁ s₂: State) (h₁: CommandEval c₁ s₁ .break s₂): CommandEval (.seq c₁ c₂) s₁ .break s₂ := by
+  theorem Arith.compile.correct (state: State) (e: Arith): e.compile.eval state Stack.empty = [e.eval state] := by
     sorry
+    where
+    helper (state: State) (stack: Stack) (e: Arith): e.compile.eval state stack = e.eval state :: stack := by
+      sorry
 
-  example (c: Logic) (b: Command) (s₁ s₂: State) (h₁: CommandEval (.while c b) s₁ .continue s₂) (h₂: c.eval s₂ = true): ∃ s₃: State, CommandEval b s₃ .break s₂ := by
-    sorry
+  @[reducible]
+  def Logic.shortCircuitEval (state: State): Logic → Bool
+    | .and e₁ e₂ =>
+      if e₁.eval state
+      then Bool.true
+      else e₂.eval state
+    | l => l.eval state
 
-  theorem CommandEval.deterministic (c: Command) (s₁ s₂ s₃: State) (r₁ r₂: Result) (h₁: CommandEval c s₁ r₁ s₂) (h₂: CommandEval c s₁ r₂ s₃): s₂ = s₃ ∧ r₁ = r₂ := by
-    sorry
-end BreakImp
+  theorem Logic.shortCircuitEval.eval (state: State) (b: Logic): b.shortCircuitEval state = b.eval state := by
+    induction b
+    <;> try rfl
+    case and e₁ e₂ h₁ h₂ =>
+      sorry
 
-namespace ForImp
-  -- TODO
-end ForImp
+  namespace BreakImp
+    inductive Command: Type where
+      | skip: Command
+      | break: Command
+      | assign (id: String) (e: Arith): Command
+      | seq (c₁ c₂: Command): Command
+      | if (b: Logic) (c₁ c₂: Command): Command
+      | while (b: Logic) (c: Command): Command
+
+    inductive Result: Type where
+      | continue: Result
+      | break: Result
+
+    inductive CommandEval: Command → State → Result → State → Prop where
+      | skip (s: State): CommandEval .skip s .continue s
+      | break (s: State): CommandEval .break s .break s
+      | assign {e: Arith} {n: Nat} {id: String} (s: State) (h: e.eval s = n): CommandEval (.assign id e) s .continue (s.update id n)
+      | seq {c₁ c₂: Command} (s₁ s₂ s₃: State) (h₁: CommandEval c₁ s₁ .continue s₂) (h₂: CommandEval c₂ s₂ .continue s₃): CommandEval (.seq c₁ c₂) s₁ .continue s₃
+      | ifTrue {c: Logic} {t f: Command} (s₁ s₂: State) (h₁: c.eval s₁ = .true) (h₂: CommandEval t s₁ .continue s₂): CommandEval (.if c t f) s₁ .continue s₂
+      | ifFalse {c: Logic} {t f: Command} (s₁ s₂: State) (h₁: c.eval s₁ = .false) (h₂: CommandEval f s₁ .continue s₂): CommandEval (.if c t f) s₁ .continue s₂
+      | whileTrue {c: Logic} {b: Command} (s₁ s₂ s₃: State) (h₁: c.eval s₁ = .true) (h₂: CommandEval b s₁ .continue s₂) (h₃: CommandEval (.while c b) s₂ .continue s₃): CommandEval (.while c b) s₁ .continue s₃
+      | whileFalse {c: Logic} {b: Command} (s: State) (h₁: c.eval s = .false): CommandEval (.while c b) s .continue s
+
+    example (c: Command) (s₁ s₂: State) (r: Result): CommandEval (.seq .break c) s₁ r s₂ := by
+      sorry
+
+    example (c: Logic) (b: Command) (s₁ s₂: State) (r: Result): CommandEval (.while c b) s₁ r s₂ := by
+      sorry
+
+    example (c: Logic) (b: Command) (s₁ s₂: State) (h₁: c.eval s₁ = true) (h₂: CommandEval b s₁ .break s₂): CommandEval (.while c b) s₁ .continue s₂ := by
+      sorry
+
+    example (c₁ c₂: Command) (s₁ s₂ s₃: State) (h₁: CommandEval c₁ s₁ .continue s₂) (h₂: CommandEval c₂ s₂ .continue s₃): CommandEval (.seq c₁ c₂) s₁ .continue s₂ := by
+      sorry
+
+    example (c₁ c₂: Command) (s₁ s₂: State) (h₁: CommandEval c₁ s₁ .break s₂): CommandEval (.seq c₁ c₂) s₁ .break s₂ := by
+      sorry
+
+    example (c: Logic) (b: Command) (s₁ s₂: State) (h₁: CommandEval (.while c b) s₁ .continue s₂) (h₂: c.eval s₂ = true): ∃ s₃: State, CommandEval b s₃ .break s₂ := by
+      sorry
+
+    theorem CommandEval.deterministic (c: Command) (s₁ s₂ s₃: State) (r₁ r₂: Result) (h₁: CommandEval c s₁ r₁ s₂) (h₂: CommandEval c s₁ r₂ s₃): s₂ = s₃ ∧ r₁ = r₂ := by
+      sorry
+  end BreakImp
+
+  namespace ForImp
+    -- TODO
+  end ForImp
+end SoftwareFoundations.LogicalFoundations.Imp
