SoftwareFoundations/LogicalFoundations/ImpCEvalFun.lean
@@ -7,88 +7,92 @@ import «SoftwareFoundations».«LogicalFoundations».«Imp»
 
 import Mathlib.Tactic.Relation.Trans
 
-/-
-## A Broken Evaluator
--/
+namespace SoftwareFoundations.LogicalFoundations.ImpCEvalFun
+  open Imp
 
-def Command.broken (state: State): Command → State
-  | .skip => state
-  | .assign id e => state.update id (e.eval state)
-  | .seq c₁ c₂ =>
-    state
-      |> c₁.broken
-      |> c₂.broken
-  | .if c t f =>
-    if c.eval state
-    then t.broken state
-    else f.broken state
-  | .while _ _ => state
+  /-
+  ## A Broken Evaluator
+  -/
 
-/-
-## A Step-Indexed Evaluator
--/
+  def _root_.SoftwareFoundations.LogicalFoundations.Imp.Command.broken (state: State): Command → State
+    | .skip => state
+    | .assign id e => state.update id (e.eval state)
+    | .seq c₁ c₂ =>
+      state
+        |> c₁.broken
+        |> c₂.broken
+    | .if c t f =>
+      if c.eval state
+      then t.broken state
+      else f.broken state
+    | .while _ _ => state
 
-def Command.eval (state: State): Nat → Command → Option State
-  | 0, _ => .none
-  | .succ _, .skip => .some state
-  | .succ _, .assign id e => .some (state.update id (e.eval state))
-  | .succ i, .seq c₁ c₂ =>
-    let state := c₁.eval state i
-    match state with
-      | .none => .none
-      | .some state => c₂.eval state i
-  | .succ i, .if c t f =>
-    if c.eval state
-    then t.eval state i
-    else f.eval state i
-  | .succ i, .while c b =>
-    if c.eval state
-    then
-      match b.eval state i with
+  /-
+  ## A Step-Indexed Evaluator
+  -/
+
+  def _root_.SoftwareFoundations.LogicalFoundations.Imp.Command.eval (state: State): Nat → Command → Option State
+    | 0, _ => .none
+    | .succ _, .skip => .some state
+    | .succ _, .assign id e => .some (state.update id (e.eval state))
+    | .succ i, .seq c₁ c₂ =>
+      let state := c₁.eval state i
+      match state with
         | .none => .none
-        | .some state => (Command.while c b).eval state i
-    else .some state
+        | .some state => c₂.eval state i
+    | .succ i, .if c t f =>
+      if c.eval state
+      then t.eval state i
+      else f.eval state i
+    | .succ i, .while c b =>
+      if c.eval state
+      then
+        match b.eval state i with
+          | .none => .none
+          | .some state => (Command.while c b).eval state i
+      else .some state
 
-def Command.eval_test (state: State) (c: Command): Option (Nat × Nat × Nat) :=
-  match c.eval state 100 with
-    | .none => .none
-    | .some state => .some (state "X", state "Y", state "Z")
+  def _root_.SoftwareFoundations.LogicalFoundations.Imp.Command.eval_test (state: State) (c: Command): Option (Nat × Nat × Nat) :=
+    match c.eval state 100 with
+      | .none => .none
+      | .some state => .some (state "X", state "Y", state "Z")
 
-example: (Command.seq (.assign "X" 2) (.if (.le "X" 1) (.assign "Y" 3) (.assign "Z" 4))).eval_test State.empty = .some (2, 0, 4) := rfl
+  example: (Command.seq (.assign "X" 2) (.if (.le "X" 1) (.assign "Y" 3) (.assign "Z" 4))).eval_test State.empty = .some (2, 0, 4) := rfl
 
--- TODO: Pup
+  -- TODO: Pup
 
-def pEven: Command :=
-  (.while (.gt "X" 1)
-    (.assign "X" (.minus "X" 2)))
+  def pEven: Command :=
+    (.while (.gt "X" 1)
+      (.assign "X" (.minus "X" 2)))
 
-example: pEven.eval_test (State.build [("X", 0)]) = .some (0, 0, 0) := rfl
-example: pEven.eval_test (State.build [("X", 1)]) = .some (1, 0, 0) := rfl
-example: pEven.eval_test (State.build [("X", 2)]) = .some (0, 0, 0) := rfl
-example: pEven.eval_test (State.build [("X", 3)]) = .some (1, 0, 0) := rfl
-example: pEven.eval_test (State.build [("X", 42)]) = .some (0, 0, 0) := rfl
-example: pEven.eval_test (State.build [("X", 43)]) = .some (1, 0, 0) := rfl
-example: pEven.eval_test (State.build [("X", 200)]) = .none := rfl
+  example: pEven.eval_test (State.build [("X", 0)]) = .some (0, 0, 0) := rfl
+  example: pEven.eval_test (State.build [("X", 1)]) = .some (1, 0, 0) := rfl
+  example: pEven.eval_test (State.build [("X", 2)]) = .some (0, 0, 0) := rfl
+  example: pEven.eval_test (State.build [("X", 3)]) = .some (1, 0, 0) := rfl
+  example: pEven.eval_test (State.build [("X", 42)]) = .some (0, 0, 0) := rfl
+  example: pEven.eval_test (State.build [("X", 43)]) = .some (1, 0, 0) := rfl
+  example: pEven.eval_test (State.build [("X", 200)]) = .none := rfl
 
-/-
-## Relational vs. Step-Indexed Evaluation
--/
+  /-
+  ## Relational vs. Step-Indexed Evaluation
+  -/
 
-theorem Command.eval.equiv_rel (c: Command) (s₁ s₂: State): (∃ i: Nat, c.eval s₁ i = .some s₂) → CommandEval c s₁ s₂ := by
-  sorry
+  theorem Command.eval.equiv_rel (c: Command) (s₁ s₂: State): (∃ i: Nat, c.eval s₁ i = .some s₂) → CommandEval c s₁ s₂ := by
+    sorry
 
-theorem Command.eval.step (c: Command) (s₁ s₂: State) (h: CommandEval c s₁ s₂): ∃ i: Nat, c.eval s₁ i = .some s₂ := by
-  sorry
-  where
-    more (i₁ i₂: Nat) (s₁ s₂: State) (c: Command) (h₁: i₁ ≤ i₂) (h₂: c.eval s₁ i₁ = s₂): c.eval s₁ i₂ = s₂ := by
-      sorry
+  theorem Command.eval.step (c: Command) (s₁ s₂: State) (h: CommandEval c s₁ s₂): ∃ i: Nat, c.eval s₁ i = .some s₂ := by
+    sorry
+    where
+      more (i₁ i₂: Nat) (s₁ s₂: State) (c: Command) (h₁: i₁ ≤ i₂) (h₂: c.eval s₁ i₁ = s₂): c.eval s₁ i₂ = s₂ := by
+        sorry
 
-theorem Command.eval.equiv_step (c: Command) (s₁ s₂: State): CommandEval c s₁ s₂ ↔ ∃ i: Nat, c.eval s₁ i = .some s₂ := by
-  sorry
+  theorem Command.eval.equiv_step (c: Command) (s₁ s₂: State): CommandEval c s₁ s₂ ↔ ∃ i: Nat, c.eval s₁ i = .some s₂ := by
+    sorry
 
-/-
-## Determinism of Evaluation Again
--/
+  /-
+  ## Determinism of Evaluation Again
+  -/
 
-theorem CommandEval.deterministic.better (c: Command) (s₁ s₂ s₃: State) (h₁: CommandEval c s₁ s₂) (h₂: CommandEval c s₁ s₃): s₂ = s₃ := by
-  sorry
+  theorem CommandEval.deterministic.better (c: Command) (s₁ s₂ s₃: State) (h₁: CommandEval c s₁ s₂) (h₂: CommandEval c s₁ s₃): s₂ = s₃ := by
+    sorry
+end SoftwareFoundations.LogicalFoundations.ImpCEvalFun
