SoftwareFoundations/LogicalFoundations/ImpParser.lean
@@ -4,111 +4,113 @@
 
 import «SoftwareFoundations».«LogicalFoundations».«Maps»
 
-/-
-## Internals
--/
+namespace SoftwareFoundations.LogicalFoundations.ImpParser
+  /-
+  ## Internals
+  -/
 
-/-
-### Lexical Analysis
--/
+  /-
+  ### Lexical Analysis
+  -/
 
-inductive CharType: Type where
-  | whitespace: CharType
-  | alpha (c: Char): CharType
-  | digit (n: Nat): CharType
-  | other (c: Char): CharType
+  inductive CharType: Type where
+    | whitespace: CharType
+    | alpha (c: Char): CharType
+    | digit (n: Nat): CharType
+    | other (c: Char): CharType
 
-def Char.classify (c: Char): CharType :=
-  if c.isWhitespace then .whitespace
-  else if c.isAlpha then .alpha c
-  else if c.isDigit then .digit c.toString.toNat!
-  else .other c
+  def Char.classify (c: Char): CharType :=
+    if c.isWhitespace then .whitespace
+    else if c.isAlpha then .alpha c
+    else if c.isDigit then .digit c.toString.toNat!
+    else .other c
 
-inductive Token: Type where
-  | semicolon: Token
-  | leftParen: Token
-  | rightParen: Token
-  | leftBracket: Token
-  | rightBracket: Token
-  | assign: Token
-  | plus: Token
-  | minus: Token
-  | times: Token
-  | eq: Token
-  | neq: Token
-  | le: Token
-  | gt: Token
-  | not: Token
-  | and: Token
-  | while: Token
-  | if: Token
-  | else: Token
-  | for: Token
-  | skip: Token
-  | break: Token
-  | true: Token
-  | false: Token
-  | id: String → Token
-  | num: Nat → Token
-deriving Repr
+  inductive Token: Type where
+    | semicolon: Token
+    | leftParen: Token
+    | rightParen: Token
+    | leftBracket: Token
+    | rightBracket: Token
+    | assign: Token
+    | plus: Token
+    | minus: Token
+    | times: Token
+    | eq: Token
+    | neq: Token
+    | le: Token
+    | gt: Token
+    | not: Token
+    | and: Token
+    | while: Token
+    | if: Token
+    | else: Token
+    | for: Token
+    | skip: Token
+    | break: Token
+    | true: Token
+    | false: Token
+    | id: String → Token
+    | num: Nat → Token
+  deriving Repr
 
--- TODO: Move `start` into loop so termination is proven
--- TODO: Make more "monadic" and use `do` syntax
--- TODO: Add CLI to run `Imp` programs
-partial def String.tokenize (s: String): Except Char (List Token) :=
-  let rec loop (acc: List Token) (cs: List CharType): Except Char (List Token) :=
-      match cs with
-        | .whitespace :: cs => loop acc cs
-        | .other ';' :: cs => loop (.semicolon :: acc) cs
-        | .other '(' :: cs => loop (.leftParen :: acc) cs
-        | .other ')' :: cs => loop (.rightParen :: acc) cs
-        | .other '{' :: cs => loop (.leftBracket :: acc) cs
-        | .other '}' :: cs => loop (.rightBracket :: acc) cs
-        | .other ':' :: .other '=' :: cs => loop (.assign :: acc) cs
-        | .other '+' :: cs => loop (.plus :: acc) cs
-        | .other '-' :: cs => loop (.minus :: acc) cs
-        | .other '*' :: cs => loop (.times :: acc) cs
-        | .other '=' :: .other '=' :: cs => loop (.eq :: acc) cs
-        | .other '!' :: .other '=' :: cs => loop (.neq :: acc) cs
-        | .other '≤' :: cs => loop (.le :: acc) cs
-        | .other '>' :: cs => loop (.gt :: acc) cs
-        | .other '~' :: cs => loop (.not :: acc) cs
-        | .other '&' :: .other '&' :: cs => loop (.and :: acc) cs
-        | .other c :: _ => Except.error c
-        | .alpha 's' :: .alpha 'k' :: .alpha 'i' :: .alpha 'p' :: cs => loop (.skip :: acc) cs
-        | .alpha 'i' :: .alpha 'f' :: cs => loop (.if :: acc) cs
-        | .alpha 'e' :: .alpha 'l' :: .alpha 's' :: .alpha 'e' :: cs => loop (.else :: acc) cs
-        | .alpha 'f' :: .alpha 'o' :: .alpha 'r' :: cs => loop (.for :: acc) cs
-        | .alpha 'w' :: .alpha 'h' :: .alpha 'i' :: .alpha 'l' :: .alpha 'e' :: cs => loop (.while :: acc) cs
-        | .alpha 'b' :: .alpha 'r' :: .alpha 'e' :: .alpha 'a' :: .alpha 'k' :: cs => loop (.break :: acc) cs
-        | .alpha 't' :: .alpha 'r' :: .alpha 'u' :: .alpha 'e' :: cs => loop (.true :: acc) cs
-        | .alpha 'f' :: .alpha 'a' :: .alpha 'l' :: .alpha 's' :: .alpha 'e' :: cs => loop (.false :: acc) cs
-        | .alpha c :: cs =>
-          let (tok, cs) := id [c] cs
-          loop (.id tok :: acc) cs
-        | .digit n :: cs =>
-          let (tok, cs) := num n cs
-          loop (.num tok :: acc) cs
-        | [] => Except.ok acc.reverse
-  loop [] (s.toList.map Char.classify)
-  where
-    id (acc: List Char) (cs: List CharType): (String × List CharType) :=
-      match cs with
-        | .alpha c :: cs => id (c :: acc) cs
-        | .digit n :: cs => id ((n.toDigits (base := 10)).reverse ++ acc) cs
-        | .other '_' :: cs => id ('_' :: acc) cs
-        | _ => (acc.reverse.asString, cs)
-    num (acc: Nat) (cs: List CharType): (Nat × List CharType) :=
-      match cs with
-        | .digit d :: cs => num (acc * 10 + d) cs
-        | _ => (acc, cs)
+  -- TODO: Move `start` into loop so termination is proven
+  -- TODO: Make more "monadic" and use `do` syntax
+  -- TODO: Add CLI to run `Imp` programs
+  partial def _root_.String.tokenize (s: String): Except Char (List Token) :=
+    let rec loop (acc: List Token) (cs: List CharType): Except Char (List Token) :=
+        match cs with
+          | .whitespace :: cs => loop acc cs
+          | .other ';' :: cs => loop (.semicolon :: acc) cs
+          | .other '(' :: cs => loop (.leftParen :: acc) cs
+          | .other ')' :: cs => loop (.rightParen :: acc) cs
+          | .other '{' :: cs => loop (.leftBracket :: acc) cs
+          | .other '}' :: cs => loop (.rightBracket :: acc) cs
+          | .other ':' :: .other '=' :: cs => loop (.assign :: acc) cs
+          | .other '+' :: cs => loop (.plus :: acc) cs
+          | .other '-' :: cs => loop (.minus :: acc) cs
+          | .other '*' :: cs => loop (.times :: acc) cs
+          | .other '=' :: .other '=' :: cs => loop (.eq :: acc) cs
+          | .other '!' :: .other '=' :: cs => loop (.neq :: acc) cs
+          | .other '≤' :: cs => loop (.le :: acc) cs
+          | .other '>' :: cs => loop (.gt :: acc) cs
+          | .other '~' :: cs => loop (.not :: acc) cs
+          | .other '&' :: .other '&' :: cs => loop (.and :: acc) cs
+          | .other c :: _ => Except.error c
+          | .alpha 's' :: .alpha 'k' :: .alpha 'i' :: .alpha 'p' :: cs => loop (.skip :: acc) cs
+          | .alpha 'i' :: .alpha 'f' :: cs => loop (.if :: acc) cs
+          | .alpha 'e' :: .alpha 'l' :: .alpha 's' :: .alpha 'e' :: cs => loop (.else :: acc) cs
+          | .alpha 'f' :: .alpha 'o' :: .alpha 'r' :: cs => loop (.for :: acc) cs
+          | .alpha 'w' :: .alpha 'h' :: .alpha 'i' :: .alpha 'l' :: .alpha 'e' :: cs => loop (.while :: acc) cs
+          | .alpha 'b' :: .alpha 'r' :: .alpha 'e' :: .alpha 'a' :: .alpha 'k' :: cs => loop (.break :: acc) cs
+          | .alpha 't' :: .alpha 'r' :: .alpha 'u' :: .alpha 'e' :: cs => loop (.true :: acc) cs
+          | .alpha 'f' :: .alpha 'a' :: .alpha 'l' :: .alpha 's' :: .alpha 'e' :: cs => loop (.false :: acc) cs
+          | .alpha c :: cs =>
+            let (tok, cs) := id [c] cs
+            loop (.id tok :: acc) cs
+          | .digit n :: cs =>
+            let (tok, cs) := num n cs
+            loop (.num tok :: acc) cs
+          | [] => Except.ok acc.reverse
+    loop [] (s.toList.map Char.classify)
+    where
+      id (acc: List Char) (cs: List CharType): (String × List CharType) :=
+        match cs with
+          | .alpha c :: cs => id (c :: acc) cs
+          | .digit n :: cs => id ((n.toDigits (base := 10)).reverse ++ acc) cs
+          | .other '_' :: cs => id ('_' :: acc) cs
+          | _ => (acc.reverse.asString, cs)
+      num (acc: Nat) (cs: List CharType): (Nat × List CharType) :=
+        match cs with
+          | .digit d :: cs => num (acc * 10 + d) cs
+          | _ => (acc, cs)
 
-#eval "".tokenize
-#eval ";(){}+-*:===!=≤>~&&skipifelseforwhilebreaktruefalse1 32asdfasdf  asfd_42_fooBar".tokenize
-#eval "   abc12=3 223*(3+(a+c))  ".tokenize
+  #eval "".tokenize
+  #eval ";(){}+-*:===!=≤>~&&skipifelseforwhilebreaktruefalse1 32asdfasdf  asfd_42_fooBar".tokenize
+  #eval "   abc12=3 223*(3+(a+c))  ".tokenize
 
-/-
-### Parsing
--/
+  /-
+  ### Parsing
+  -/
 
-def Parser (τ: Type) (ε: Type) (σ: Type): Type := List τ → Except ε σ
+  def Parser (τ: Type) (ε: Type) (σ: Type): Type := List τ → Except ε σ
+end SoftwareFoundations.LogicalFoundations.ImpParser
