SoftwareFoundations/LogicalFoundations/Maps.lean
@@ -2,118 +2,120 @@
 # Total and Partial Maps
 -/
 
-/-
-## Identifiers
--/
+namespace SoftwareFoundations.LogicalFoundations.Maps
+  /-
+  ## Identifiers
+  -/
 
-#check BEq String
+  #check BEq String
 
-/-
-## Total Maps
--/
+  /-
+  ## Total Maps
+  -/
 
-def TotalMap (α: Type): Type := String → α
+  def TotalMap (α: Type): Type := String → α
 
-def TotalMap.empty {α: Type} (default: α): TotalMap α := fun _ => default
+  def TotalMap.empty {α: Type} (default: α): TotalMap α := fun _ => default
 
-@[reducible]
-def TotalMap.update {α: Type} (m: TotalMap α) (k: String) (v: α): TotalMap α :=
-  fun k₁ =>
-    if k == k₁
-    then v
-    else m k₁
+  @[reducible]
+  def TotalMap.update {α: Type} (m: TotalMap α) (k: String) (v: α): TotalMap α :=
+    fun k₁ =>
+      if k == k₁
+      then v
+      else m k₁
 
-example: TotalMap Bool :=
-  ((TotalMap.empty false).update "foo" true).update "bar" true
+  example: TotalMap Bool :=
+    ((TotalMap.empty false).update "foo" true).update "bar" true
 
-@[simp]
-theorem TotalMap.applyEmpty (k: String) (v: α): (TotalMap.empty v) k = v := by rfl
+  @[simp]
+  theorem TotalMap.applyEmpty (k: String) (v: α): (TotalMap.empty v) k = v := by rfl
 
-@[simp]
-theorem TotalMap.updateEq (m: TotalMap α) (k: String) (v: α): (m.update k v) k = v := by
-  unfold TotalMap.update
-  simp
+  @[simp]
+  theorem TotalMap.updateEq (m: TotalMap α) (k: String) (v: α): (m.update k v) k = v := by
+    unfold TotalMap.update
+    simp
 
-@[simp]
-theorem TotalMap.updateNeq (m: TotalMap α) (k₁ k₂: String) (v: α) (h: k₁ ≠ k₂): (m.update k₁ v) k₂ = m k₂ := by
-  unfold TotalMap.update
-  simp_all
+  @[simp]
+  theorem TotalMap.updateNeq (m: TotalMap α) (k₁ k₂: String) (v: α) (h: k₁ ≠ k₂): (m.update k₁ v) k₂ = m k₂ := by
+    unfold TotalMap.update
+    simp_all
 
-@[simp]
-theorem TotalMap.updateShadow (m: TotalMap α) (k: String) (v₁ v₂: α): ((m.update k v₁).update k v₂) k = (m.update k v₂) k := by
-  unfold TotalMap.update
-  simp
+  @[simp]
+  theorem TotalMap.updateShadow (m: TotalMap α) (k: String) (v₁ v₂: α): ((m.update k v₁).update k v₂) k = (m.update k v₂) k := by
+    unfold TotalMap.update
+    simp
 
-@[simp]
-theorem TotalMap.updateSame (m: TotalMap α) (k: String): (m.update k (m k)) = m := by
-  unfold TotalMap.update
-  funext x
-  cases k == x with
-    | true =>
-      simp
-      congr
-      sorry
-    | false => simp
+  @[simp]
+  theorem TotalMap.updateSame (m: TotalMap α) (k: String): (m.update k (m k)) = m := by
+    unfold TotalMap.update
+    funext x
+    cases k == x with
+      | true =>
+        simp
+        congr
+        sorry
+      | false => simp
 
-theorem TotalMap.updatePermute (m: TotalMap α) (k₁ k₂: String) (v₁ v₂: α) (h: k₁ ≠ k₂): (m.update k₁ v₁).update k₂ v₂ = (m.update k₂ v₂).update k₁ v₁ := by
-  simp at *
-  unfold TotalMap.update
-  funext x
-  cases k₁ == x with
-    | true =>
-      cases k₂ == x with
-        | true => simp; sorry
-        | false => simp
-    | false =>
-      cases k₂ == x with
-        | true => simp
-        | false => simp
+  theorem TotalMap.updatePermute (m: TotalMap α) (k₁ k₂: String) (v₁ v₂: α) (h: k₁ ≠ k₂): (m.update k₁ v₁).update k₂ v₂ = (m.update k₂ v₂).update k₁ v₁ := by
+    simp at *
+    unfold TotalMap.update
+    funext x
+    cases k₁ == x with
+      | true =>
+        cases k₂ == x with
+          | true => simp; sorry
+          | false => simp
+      | false =>
+        cases k₂ == x with
+          | true => simp
+          | false => simp
 
-/-
-## Partial Maps
--/
+  /-
+  ## Partial Maps
+  -/
 
-def PartialMap (α: Type): Type := TotalMap (Option α)
+  def PartialMap (α: Type): Type := TotalMap (Option α)
 
-def PartialMap.empty: PartialMap α := TotalMap.empty .none
+  def PartialMap.empty: PartialMap α := TotalMap.empty .none
 
-@[reducible]
-def PartialMap.update (m: PartialMap α) (k: String) (v: α): PartialMap α := TotalMap.update m k v
+  @[reducible]
+  def PartialMap.update (m: PartialMap α) (k: String) (v: α): PartialMap α := TotalMap.update m k v
 
-def PartialMap.includes (m₁ m₂: PartialMap α): Prop := ∀ k: String, ∀ v: α, m₁ k = .some v → m₂ k = .some v
+  def PartialMap.includes (m₁ m₂: PartialMap α): Prop := ∀ k: String, ∀ v: α, m₁ k = .some v → m₂ k = .some v
 
-theorem PartialMap.applyEmpty (k: String): @PartialMap.empty α k = .none := by rfl
+  theorem PartialMap.applyEmpty (k: String): @PartialMap.empty α k = .none := by rfl
 
-@[simp]
-theorem PartialMap.updateEq (m: PartialMap α) (k: String) (v: α): (m.update k v) k = v := by
-  unfold PartialMap.update
-  rw [TotalMap.updateEq]
+  @[simp]
+  theorem PartialMap.updateEq (m: PartialMap α) (k: String) (v: α): (m.update k v) k = v := by
+    unfold PartialMap.update
+    rw [TotalMap.updateEq]
 
-@[simp]
-theorem PartialMap.updateNeq (m: PartialMap α) (k₁ k₂: String) (v: α) (h: k₁ ≠ k₂): (m.update k₁ v) k₂ = m k₂ := by
-  unfold PartialMap.update
-  rw [TotalMap.updateNeq]
-  assumption
+  @[simp]
+  theorem PartialMap.updateNeq (m: PartialMap α) (k₁ k₂: String) (v: α) (h: k₁ ≠ k₂): (m.update k₁ v) k₂ = m k₂ := by
+    unfold PartialMap.update
+    rw [TotalMap.updateNeq]
+    assumption
 
-@[simp]
-theorem PartialMap.updateShadow (m: PartialMap α) (k: String) (v₁ v₂: α): ((m.update k v₁).update k v₂) k = (m.update k v₂) k := by
-  unfold PartialMap.update
-  rw [TotalMap.updateShadow]
+  @[simp]
+  theorem PartialMap.updateShadow (m: PartialMap α) (k: String) (v₁ v₂: α): ((m.update k v₁).update k v₂) k = (m.update k v₂) k := by
+    unfold PartialMap.update
+    rw [TotalMap.updateShadow]
 
-@[simp]
-theorem PartialMap.updateSame (m: PartialMap α) (k: String) (v: α) (h: m k = .some v): (m.update k v) = m := by
-  unfold PartialMap.update
-  rw [← h]
-  rw [TotalMap.updateSame]
+  @[simp]
+  theorem PartialMap.updateSame (m: PartialMap α) (k: String) (v: α) (h: m k = .some v): (m.update k v) = m := by
+    unfold PartialMap.update
+    rw [← h]
+    rw [TotalMap.updateSame]
 
-theorem PartialMap.updatePermute (m: PartialMap α) (k₁ k₂: String) (v₁ v₂: α) (h: k₁ ≠ k₂): (m.update k₁ v₁).update k₂ v₂ = (m.update k₂ v₂).update k₁ v₁ := by
-  unfold PartialMap.update
-  rw [TotalMap.updatePermute]
-  assumption
+  theorem PartialMap.updatePermute (m: PartialMap α) (k₁ k₂: String) (v₁ v₂: α) (h: k₁ ≠ k₂): (m.update k₁ v₁).update k₂ v₂ = (m.update k₂ v₂).update k₁ v₁ := by
+    unfold PartialMap.update
+    rw [TotalMap.updatePermute]
+    assumption
 
-theorem PartialMap.includesUpdate (m₁ m₂: PartialMap α) (k: String) (v: α) (h: m₁.includes m₂): (m₁.update k v).includes (m₂.update k v) := by
-  unfold PartialMap.includes
-  intro k₁ v₁ h₂
-  cases k == k₁ with
-    | true =>sorry
-    | false => sorry
+  theorem PartialMap.includesUpdate (m₁ m₂: PartialMap α) (k: String) (v: α) (h: m₁.includes m₂): (m₁.update k v).includes (m₂.update k v) := by
+    unfold PartialMap.includes
+    intro k₁ v₁ h₂
+    cases k == k₁ with
+      | true => sorry
+      | false => sorry
+end SoftwareFoundations.LogicalFoundations.Maps
